git/Augustindou/natural2lean/src/natural2lean/proof_elements/statement/__init__.py
@@ -1,12 +1,13 @@
+from natural2lean.proof_elements.statement.such_that import SuchThat
 from .have import Have
-from .such_that import SuchThat
+from .proof_structure import ProofStructure
 from .statement import Statement
 from ...propositions.multiple_propositions import MultiplePropositions
 from ...utils.exceptions import MatchingError, TranslationError
 
-POSSIBILITIES = [Have, SuchThat]
+POSSIBILITIES = [Have, ProofStructure]
 # conclusions, statements that would only be accepted if they are conclusions of a goal
-CCL_POSSIBILITIES = [MultiplePropositions]
+CCL_POSSIBILITIES = [MultiplePropositions, SuchThat]
 
 
 def get_statement(string: str) -> Statement:
@@ -17,6 +18,6 @@ def get_statement(string: str) -> Statement:
             pass
 
     raise TranslationError(
-        f"Could not match any statement for {string}, tried "
+        f"Could not match any statement for '{string}', tried "
         + ", ".join([p.__name__ for p in POSSIBILITIES])
     )
