git/leanprover/lean4/stage0/stdlib/Lean/Data/Lsp/Extra.c
@@ -105,7 +105,7 @@ static lean_object* l___private_Lean_Data_Lsp_Extra_0__Lean_Lsp_fromJsonLeanFile
 LEAN_EXPORT lean_object* l___private_Lean_Data_Lsp_Extra_0__Lean_Lsp_fromJsonWaitForDiagnosticsParams____x40_Lean_Data_Lsp_Extra___hyg_24_(lean_object*);
 uint8_t lean_nat_dec_eq(lean_object*, lean_object*);
 static lean_object* l_Lean_Lsp_instToJsonLeanFileProgressKind___closed__2;
-lean_object* l_Lean_Json_getObjValAs_x3f___at___private_Lean_Data_Lsp_Basic_0__Lean_Lsp_fromJsonTextDocumentPositionParams____x40_Lean_Data_Lsp_Basic___hyg_1983____spec__1(lean_object*, lean_object*);
+lean_object* l_Lean_Json_getObjValAs_x3f___at___private_Lean_Data_Lsp_Basic_0__Lean_Lsp_fromJsonTextDocumentPositionParams____x40_Lean_Data_Lsp_Basic___hyg_1974____spec__1(lean_object*, lean_object*);
 lean_object* l_Lean_bignumToJson(lean_object*);
 static lean_object* l_Lean_Lsp_instFromJsonLeanFileProgressKind___closed__2;
 LEAN_EXPORT lean_object* l___private_Lean_Data_Lsp_Extra_0__Lean_Lsp_toJsonRpcConnected____x40_Lean_Data_Lsp_Extra___hyg_1190____boxed(lean_object*);
@@ -171,7 +171,7 @@ static lean_object* l_Lean_Json_getObjValAs_x3f___at___private_Lean_Data_Lsp_Ext
 LEAN_EXPORT lean_object* l___private_Lean_Data_Lsp_Extra_0__Lean_Lsp_beqLeanFileProgressKind____x40_Lean_Data_Lsp_Extra___hyg_151____boxed(lean_object*, lean_object*);
 static lean_object* l___private_Lean_Data_Lsp_Extra_0__Lean_Lsp_reprLineRange____x40_Lean_Data_Lsp_Extra___hyg_1718____closed__6;
 LEAN_EXPORT lean_object* l_Lean_Json_getObjValAs_x3f___at___private_Lean_Data_Lsp_Extra_0__Lean_Lsp_fromJsonLeanFileProgressProcessingInfo____x40_Lean_Data_Lsp_Extra___hyg_267____spec__1(lean_object*, lean_object*);
-lean_object* l___private_Lean_Data_Lsp_Basic_0__Lean_Lsp_toJsonTextDocumentIdentifier____x40_Lean_Data_Lsp_Basic___hyg_1457_(lean_object*);
+lean_object* l___private_Lean_Data_Lsp_Basic_0__Lean_Lsp_toJsonTextDocumentIdentifier____x40_Lean_Data_Lsp_Basic___hyg_1451_(lean_object*);
 LEAN_EXPORT lean_object* l_Array_mapMUnsafe_map___at___private_Lean_Data_Lsp_Extra_0__Lean_Lsp_toJsonPlainGoal____x40_Lean_Data_Lsp_Extra___hyg_646____spec__1___boxed(lean_object*, lean_object*, lean_object*);
 LEAN_EXPORT lean_object* l_Lean_Lsp_instFromJsonLeanFileProgressProcessingInfo;
 LEAN_EXPORT lean_object* l_Lean_Lsp_instToJsonWaitForDiagnostics(lean_object*);
@@ -223,6 +223,7 @@ extern lean_object* l_USize_size;
 LEAN_EXPORT lean_object* l___private_Lean_Data_Lsp_Extra_0__Lean_Lsp_toJsonRpcKeepAliveParams____x40_Lean_Data_Lsp_Extra___hyg_1649_(lean_object*);
 static lean_object* l___private_Lean_Data_Lsp_Extra_0__Lean_Lsp_toJsonLeanFileProgressProcessingInfo____x40_Lean_Data_Lsp_Extra___hyg_319____closed__5;
 lean_object* l_Lean_Syntax_decodeNameLit(lean_object*);
+lean_object* l_Lean_Json_getObjValAs_x3f___at___private_Lean_Data_Lsp_Basic_0__Lean_Lsp_fromJsonTextDocumentEdit____x40_Lean_Data_Lsp_Basic___hyg_1680____spec__1(lean_object*, lean_object*);
 LEAN_EXPORT lean_object* l___private_Lean_Data_Lsp_Extra_0__Lean_Lsp_toJsonLeanFileProgressParams____x40_Lean_Data_Lsp_Extra___hyg_431_(lean_object*);
 LEAN_EXPORT lean_object* l_Array_mapMUnsafe_map___at___private_Lean_Data_Lsp_Extra_0__Lean_Lsp_toJsonLeanFileProgressParams____x40_Lean_Data_Lsp_Extra___hyg_431____spec__1(size_t, size_t, lean_object*);
 LEAN_EXPORT lean_object* l_Lean_Json_getObjValAs_x3f___at___private_Lean_Data_Lsp_Extra_0__Lean_Lsp_fromJsonRpcCallParams____x40_Lean_Data_Lsp_Extra___hyg_1254____spec__2(lean_object*, lean_object*);
@@ -249,7 +250,7 @@ static lean_object* l___private_Lean_Data_Lsp_Extra_0__Lean_Lsp_fromJsonPlainGoa
 LEAN_EXPORT lean_object* l___private_Lean_Data_Lsp_Extra_0__Lean_Lsp_toJsonRpcConnectParams____x40_Lean_Data_Lsp_Extra___hyg_1115_(lean_object*);
 static lean_object* l___private_Lean_Data_Lsp_Extra_0__Lean_Lsp_fromJsonLeanFileProgressParams____x40_Lean_Data_Lsp_Extra___hyg_379____closed__2;
 lean_object* lean_usize_to_nat(size_t);
-lean_object* l___private_Lean_Data_Lsp_Basic_0__Lean_Lsp_toJsonVersionedTextDocumentIdentifier____x40_Lean_Data_Lsp_Basic___hyg_1542_(lean_object*);
+lean_object* l___private_Lean_Data_Lsp_Basic_0__Lean_Lsp_toJsonVersionedTextDocumentIdentifier____x40_Lean_Data_Lsp_Basic___hyg_1536_(lean_object*);
 static lean_object* l___private_Lean_Data_Lsp_Extra_0__Lean_Lsp_reprLineRange____x40_Lean_Data_Lsp_Extra___hyg_1718____closed__12;
 LEAN_EXPORT lean_object* l___private_Lean_Data_Lsp_Extra_0__Lean_Lsp_fromJsonLeanFileProgressParams____x40_Lean_Data_Lsp_Extra___hyg_379_(lean_object*);
 LEAN_EXPORT lean_object* l___private_Lean_Data_Lsp_Extra_0__Lean_Lsp_toJsonRpcConnected____x40_Lean_Data_Lsp_Extra___hyg_1190_(uint64_t);
@@ -269,7 +270,6 @@ LEAN_EXPORT lean_object* l_Lean_Json_getObjValAs_x3f___at___private_Lean_Data_Ls
 lean_object* lean_nat_to_int(lean_object*);
 LEAN_EXPORT lean_object* l_Lean_Lsp_instToJsonPlainTermGoal;
 LEAN_EXPORT lean_object* l___private_Lean_Data_Lsp_Extra_0__Lean_Lsp_fromJsonLineRange____x40_Lean_Data_Lsp_Extra___hyg_1759_(lean_object*);
-lean_object* l_Lean_Json_getObjValAs_x3f___at___private_Lean_Data_Lsp_Basic_0__Lean_Lsp_fromJsonTextDocumentEdit____x40_Lean_Data_Lsp_Basic___hyg_1689____spec__1(lean_object*, lean_object*);
 LEAN_EXPORT lean_object* l_Lean_Lsp_instFromJsonRpcReleaseParams;
 static lean_object* l_Lean_Lsp_instToJsonPlainTermGoalParams___closed__1;
 LEAN_EXPORT lean_object* l_Lean_Lsp_instToJsonPlainTermGoalParams;
@@ -281,7 +281,7 @@ static lean_object* _init_l___private_Lean_Data_Lsp_Extra_0__Lean_Lsp_fromJsonWa
 _start:
 {
 lean_object* x_1; 
-x_1 = lean_mk_string("uri");
+x_1 = lean_mk_string_from_bytes("uri", 3);
 return x_1;
 }
 }
@@ -289,7 +289,7 @@ static lean_object* _init_l___private_Lean_Data_Lsp_Extra_0__Lean_Lsp_fromJsonWa
 _start:
 {
 lean_object* x_1; 
-x_1 = lean_mk_string("version");
+x_1 = lean_mk_string_from_bytes("version", 7);
 return x_1;
 }
 }
@@ -694,7 +694,7 @@ static lean_object* _init_l_Lean_Lsp_instFromJsonLeanFileProgressKind___closed__
 _start:
 {
 lean_object* x_1; 
-x_1 = lean_mk_string("unknown LeanFileProgressKind '");
+x_1 = lean_mk_string_from_bytes("unknown LeanFileProgressKind '", 30);
 return x_1;
 }
 }
@@ -702,7 +702,7 @@ static lean_object* _init_l_Lean_Lsp_instFromJsonLeanFileProgressKind___closed__
 _start:
 {
 lean_object* x_1; 
-x_1 = lean_mk_string("'");
+x_1 = lean_mk_string_from_bytes("'", 1);
 return x_1;
 }
 }
@@ -1080,7 +1080,7 @@ static lean_object* _init_l___private_Lean_Data_Lsp_Extra_0__Lean_Lsp_fromJsonLe
 _start:
 {
 lean_object* x_1; 
-x_1 = lean_mk_string("range");
+x_1 = lean_mk_string_from_bytes("range", 5);
 return x_1;
 }
 }
@@ -1088,7 +1088,7 @@ static lean_object* _init_l___private_Lean_Data_Lsp_Extra_0__Lean_Lsp_fromJsonLe
 _start:
 {
 lean_object* x_1; 
-x_1 = lean_mk_string("kind");
+x_1 = lean_mk_string_from_bytes("kind", 4);
 return x_1;
 }
 }
@@ -1404,7 +1404,7 @@ static lean_object* _init_l_Lean_Json_getObjValAs_x3f___at___private_Lean_Data_L
 _start:
 {
 lean_object* x_1; 
-x_1 = lean_mk_string("expected JSON array, got '");
+x_1 = lean_mk_string_from_bytes("expected JSON array, got '", 26);
 return x_1;
 }
 }
@@ -1448,7 +1448,7 @@ static lean_object* _init_l___private_Lean_Data_Lsp_Extra_0__Lean_Lsp_fromJsonLe
 _start:
 {
 lean_object* x_1; 
-x_1 = lean_mk_string("textDocument");
+x_1 = lean_mk_string_from_bytes("textDocument", 12);
 return x_1;
 }
 }
@@ -1456,7 +1456,7 @@ static lean_object* _init_l___private_Lean_Data_Lsp_Extra_0__Lean_Lsp_fromJsonLe
 _start:
 {
 lean_object* x_1; 
-x_1 = lean_mk_string("processing");
+x_1 = lean_mk_string_from_bytes("processing", 10);
 return x_1;
 }
 }
@@ -1465,7 +1465,7 @@ _start:
 {
 lean_object* x_2; lean_object* x_3; 
 x_2 = l___private_Lean_Data_Lsp_Extra_0__Lean_Lsp_fromJsonLeanFileProgressParams____x40_Lean_Data_Lsp_Extra___hyg_379____closed__1;
-x_3 = l_Lean_Json_getObjValAs_x3f___at___private_Lean_Data_Lsp_Basic_0__Lean_Lsp_fromJsonTextDocumentEdit____x40_Lean_Data_Lsp_Basic___hyg_1689____spec__1(x_1, x_2);
+x_3 = l_Lean_Json_getObjValAs_x3f___at___private_Lean_Data_Lsp_Basic_0__Lean_Lsp_fromJsonTextDocumentEdit____x40_Lean_Data_Lsp_Basic___hyg_1680____spec__1(x_1, x_2);
 if (lean_obj_tag(x_3) == 0)
 {
 uint8_t x_4; 
@@ -1604,8 +1604,7 @@ _start:
 lean_object* x_2; lean_object* x_3; lean_object* x_4; lean_object* x_5; lean_object* x_6; lean_object* x_7; lean_object* x_8; lean_object* x_9; size_t x_10; size_t x_11; lean_object* x_12; lean_object* x_13; lean_object* x_14; lean_object* x_15; lean_object* x_16; lean_object* x_17; lean_object* x_18; lean_object* x_19; lean_object* x_20; 
 x_2 = lean_ctor_get(x_1, 0);
 lean_inc(x_2);
-x_3 = l___private_Lean_Data_Lsp_Basic_0__Lean_Lsp_toJsonVersionedTextDocumentIdentifier____x40_Lean_Data_Lsp_Basic___hyg_1542_(x_2);
-lean_dec(x_2);
+x_3 = l___private_Lean_Data_Lsp_Basic_0__Lean_Lsp_toJsonVersionedTextDocumentIdentifier____x40_Lean_Data_Lsp_Basic___hyg_1536_(x_2);
 x_4 = l___private_Lean_Data_Lsp_Extra_0__Lean_Lsp_fromJsonLeanFileProgressParams____x40_Lean_Data_Lsp_Extra___hyg_379____closed__1;
 x_5 = lean_alloc_ctor(0, 2, 0);
 lean_ctor_set(x_5, 0, x_4);
@@ -1674,7 +1673,7 @@ static lean_object* _init_l___private_Lean_Data_Lsp_Extra_0__Lean_Lsp_fromJsonPl
 _start:
 {
 lean_object* x_1; 
-x_1 = lean_mk_string("position");
+x_1 = lean_mk_string_from_bytes("position", 8);
 return x_1;
 }
 }
@@ -1683,7 +1682,7 @@ _start:
 {
 lean_object* x_2; lean_object* x_3; 
 x_2 = l___private_Lean_Data_Lsp_Extra_0__Lean_Lsp_fromJsonLeanFileProgressParams____x40_Lean_Data_Lsp_Extra___hyg_379____closed__1;
-x_3 = l_Lean_Json_getObjValAs_x3f___at___private_Lean_Data_Lsp_Basic_0__Lean_Lsp_fromJsonTextDocumentPositionParams____x40_Lean_Data_Lsp_Basic___hyg_1983____spec__1(x_1, x_2);
+x_3 = l_Lean_Json_getObjValAs_x3f___at___private_Lean_Data_Lsp_Basic_0__Lean_Lsp_fromJsonTextDocumentPositionParams____x40_Lean_Data_Lsp_Basic___hyg_1974____spec__1(x_1, x_2);
 if (lean_obj_tag(x_3) == 0)
 {
 uint8_t x_4; 
@@ -1793,7 +1792,7 @@ _start:
 lean_object* x_2; lean_object* x_3; lean_object* x_4; lean_object* x_5; lean_object* x_6; lean_object* x_7; lean_object* x_8; lean_object* x_9; lean_object* x_10; lean_object* x_11; lean_object* x_12; lean_object* x_13; lean_object* x_14; lean_object* x_15; lean_object* x_16; 
 x_2 = lean_ctor_get(x_1, 0);
 lean_inc(x_2);
-x_3 = l___private_Lean_Data_Lsp_Basic_0__Lean_Lsp_toJsonTextDocumentIdentifier____x40_Lean_Data_Lsp_Basic___hyg_1457_(x_2);
+x_3 = l___private_Lean_Data_Lsp_Basic_0__Lean_Lsp_toJsonTextDocumentIdentifier____x40_Lean_Data_Lsp_Basic___hyg_1451_(x_2);
 x_4 = l___private_Lean_Data_Lsp_Extra_0__Lean_Lsp_fromJsonLeanFileProgressParams____x40_Lean_Data_Lsp_Extra___hyg_379____closed__1;
 x_5 = lean_alloc_ctor(0, 2, 0);
 lean_ctor_set(x_5, 0, x_4);
@@ -1936,7 +1935,7 @@ static lean_object* _init_l___private_Lean_Data_Lsp_Extra_0__Lean_Lsp_fromJsonPl
 _start:
 {
 lean_object* x_1; 
-x_1 = lean_mk_string("rendered");
+x_1 = lean_mk_string_from_bytes("rendered", 8);
 return x_1;
 }
 }
@@ -1944,7 +1943,7 @@ static lean_object* _init_l___private_Lean_Data_Lsp_Extra_0__Lean_Lsp_fromJsonPl
 _start:
 {
 lean_object* x_1; 
-x_1 = lean_mk_string("goals");
+x_1 = lean_mk_string_from_bytes("goals", 5);
 return x_1;
 }
 }
@@ -2164,7 +2163,7 @@ _start:
 {
 lean_object* x_2; lean_object* x_3; 
 x_2 = l___private_Lean_Data_Lsp_Extra_0__Lean_Lsp_fromJsonLeanFileProgressParams____x40_Lean_Data_Lsp_Extra___hyg_379____closed__1;
-x_3 = l_Lean_Json_getObjValAs_x3f___at___private_Lean_Data_Lsp_Basic_0__Lean_Lsp_fromJsonTextDocumentPositionParams____x40_Lean_Data_Lsp_Basic___hyg_1983____spec__1(x_1, x_2);
+x_3 = l_Lean_Json_getObjValAs_x3f___at___private_Lean_Data_Lsp_Basic_0__Lean_Lsp_fromJsonTextDocumentPositionParams____x40_Lean_Data_Lsp_Basic___hyg_1974____spec__1(x_1, x_2);
 if (lean_obj_tag(x_3) == 0)
 {
 uint8_t x_4; 
@@ -2274,7 +2273,7 @@ _start:
 lean_object* x_2; lean_object* x_3; lean_object* x_4; lean_object* x_5; lean_object* x_6; lean_object* x_7; lean_object* x_8; lean_object* x_9; lean_object* x_10; lean_object* x_11; lean_object* x_12; lean_object* x_13; lean_object* x_14; lean_object* x_15; lean_object* x_16; 
 x_2 = lean_ctor_get(x_1, 0);
 lean_inc(x_2);
-x_3 = l___private_Lean_Data_Lsp_Basic_0__Lean_Lsp_toJsonTextDocumentIdentifier____x40_Lean_Data_Lsp_Basic___hyg_1457_(x_2);
+x_3 = l___private_Lean_Data_Lsp_Basic_0__Lean_Lsp_toJsonTextDocumentIdentifier____x40_Lean_Data_Lsp_Basic___hyg_1451_(x_2);
 x_4 = l___private_Lean_Data_Lsp_Extra_0__Lean_Lsp_fromJsonLeanFileProgressParams____x40_Lean_Data_Lsp_Extra___hyg_379____closed__1;
 x_5 = lean_alloc_ctor(0, 2, 0);
 lean_ctor_set(x_5, 0, x_4);
@@ -2325,7 +2324,7 @@ static lean_object* _init_l___private_Lean_Data_Lsp_Extra_0__Lean_Lsp_fromJsonPl
 _start:
 {
 lean_object* x_1; 
-x_1 = lean_mk_string("goal");
+x_1 = lean_mk_string_from_bytes("goal", 4);
 return x_1;
 }
 }
@@ -2581,7 +2580,7 @@ static lean_object* _init_l_Lean_Json_getObjValAs_x3f___at___private_Lean_Data_L
 _start:
 {
 lean_object* x_1; 
-x_1 = lean_mk_string("value '{j}' is too large for `USize`");
+x_1 = lean_mk_string_from_bytes("value '{j}' is too large for `USize`", 36);
 return x_1;
 }
 }
@@ -2652,7 +2651,7 @@ static lean_object* _init_l___private_Lean_Data_Lsp_Extra_0__Lean_Lsp_fromJsonRp
 _start:
 {
 lean_object* x_1; 
-x_1 = lean_mk_string("p");
+x_1 = lean_mk_string_from_bytes("p", 1);
 return x_1;
 }
 }
@@ -2919,7 +2918,7 @@ static lean_object* _init_l_Lean_Json_getObjValAs_x3f___at___private_Lean_Data_L
 _start:
 {
 lean_object* x_1; 
-x_1 = lean_mk_string("value '{j}' is too large for `UInt64`");
+x_1 = lean_mk_string_from_bytes("value '{j}' is too large for `UInt64`", 37);
 return x_1;
 }
 }
@@ -2990,7 +2989,7 @@ static lean_object* _init_l___private_Lean_Data_Lsp_Extra_0__Lean_Lsp_fromJsonRp
 _start:
 {
 lean_object* x_1; 
-x_1 = lean_mk_string("sessionId");
+x_1 = lean_mk_string_from_bytes("sessionId", 9);
 return x_1;
 }
 }
@@ -3118,7 +3117,7 @@ static lean_object* _init_l_Lean_Json_getObjValAs_x3f___at___private_Lean_Data_L
 _start:
 {
 lean_object* x_1; 
-x_1 = lean_mk_string("[anonymous]");
+x_1 = lean_mk_string_from_bytes("[anonymous]", 11);
 return x_1;
 }
 }
@@ -3126,7 +3125,7 @@ static lean_object* _init_l_Lean_Json_getObjValAs_x3f___at___private_Lean_Data_L
 _start:
 {
 lean_object* x_1; 
-x_1 = lean_mk_string("`");
+x_1 = lean_mk_string_from_bytes("`", 1);
 return x_1;
 }
 }
@@ -3134,7 +3133,7 @@ static lean_object* _init_l_Lean_Json_getObjValAs_x3f___at___private_Lean_Data_L
 _start:
 {
 lean_object* x_1; 
-x_1 = lean_mk_string("expected a `Name`, got '");
+x_1 = lean_mk_string_from_bytes("expected a `Name`, got '", 24);
 return x_1;
 }
 }
@@ -3293,7 +3292,7 @@ static lean_object* _init_l___private_Lean_Data_Lsp_Extra_0__Lean_Lsp_fromJsonRp
 _start:
 {
 lean_object* x_1; 
-x_1 = lean_mk_string("method");
+x_1 = lean_mk_string_from_bytes("method", 6);
 return x_1;
 }
 }
@@ -3301,7 +3300,7 @@ static lean_object* _init_l___private_Lean_Data_Lsp_Extra_0__Lean_Lsp_fromJsonRp
 _start:
 {
 lean_object* x_1; 
-x_1 = lean_mk_string("params");
+x_1 = lean_mk_string_from_bytes("params", 6);
 return x_1;
 }
 }
@@ -3310,7 +3309,7 @@ _start:
 {
 lean_object* x_2; lean_object* x_3; 
 x_2 = l___private_Lean_Data_Lsp_Extra_0__Lean_Lsp_fromJsonLeanFileProgressParams____x40_Lean_Data_Lsp_Extra___hyg_379____closed__1;
-x_3 = l_Lean_Json_getObjValAs_x3f___at___private_Lean_Data_Lsp_Basic_0__Lean_Lsp_fromJsonTextDocumentPositionParams____x40_Lean_Data_Lsp_Basic___hyg_1983____spec__1(x_1, x_2);
+x_3 = l_Lean_Json_getObjValAs_x3f___at___private_Lean_Data_Lsp_Basic_0__Lean_Lsp_fromJsonTextDocumentPositionParams____x40_Lean_Data_Lsp_Basic___hyg_1974____spec__1(x_1, x_2);
 if (lean_obj_tag(x_3) == 0)
 {
 uint8_t x_4; 
@@ -3519,7 +3518,7 @@ x_2 = lean_ctor_get(x_1, 0);
 lean_inc(x_2);
 x_3 = lean_ctor_get(x_2, 0);
 lean_inc(x_3);
-x_4 = l___private_Lean_Data_Lsp_Basic_0__Lean_Lsp_toJsonTextDocumentIdentifier____x40_Lean_Data_Lsp_Basic___hyg_1457_(x_3);
+x_4 = l___private_Lean_Data_Lsp_Basic_0__Lean_Lsp_toJsonTextDocumentIdentifier____x40_Lean_Data_Lsp_Basic___hyg_1451_(x_3);
 x_5 = l___private_Lean_Data_Lsp_Extra_0__Lean_Lsp_fromJsonLeanFileProgressParams____x40_Lean_Data_Lsp_Extra___hyg_379____closed__1;
 x_6 = lean_alloc_ctor(0, 2, 0);
 lean_ctor_set(x_6, 0, x_5);
@@ -3703,7 +3702,7 @@ static lean_object* _init_l___private_Lean_Data_Lsp_Extra_0__Lean_Lsp_fromJsonRp
 _start:
 {
 lean_object* x_1; 
-x_1 = lean_mk_string("refs");
+x_1 = lean_mk_string_from_bytes("refs", 4);
 return x_1;
 }
 }
@@ -4160,7 +4159,7 @@ static lean_object* _init_l___private_Lean_Data_Lsp_Extra_0__Lean_Lsp_reprLineRa
 _start:
 {
 lean_object* x_1; 
-x_1 = lean_mk_string("start");
+x_1 = lean_mk_string_from_bytes("start", 5);
 return x_1;
 }
 }
@@ -4190,7 +4189,7 @@ static lean_object* _init_l___private_Lean_Data_Lsp_Extra_0__Lean_Lsp_reprLineRa
 _start:
 {
 lean_object* x_1; 
-x_1 = lean_mk_string(" := ");
+x_1 = lean_mk_string_from_bytes(" := ", 4);
 return x_1;
 }
 }
@@ -4220,7 +4219,7 @@ static lean_object* _init_l___private_Lean_Data_Lsp_Extra_0__Lean_Lsp_reprLineRa
 _start:
 {
 lean_object* x_1; 
-x_1 = lean_mk_string(",");
+x_1 = lean_mk_string_from_bytes(",", 1);
 return x_1;
 }
 }
@@ -4238,7 +4237,7 @@ static lean_object* _init_l___private_Lean_Data_Lsp_Extra_0__Lean_Lsp_reprLineRa
 _start:
 {
 lean_object* x_1; 
-x_1 = lean_mk_string("end");
+x_1 = lean_mk_string_from_bytes("end", 3);
 return x_1;
 }
 }
@@ -4256,7 +4255,7 @@ static lean_object* _init_l___private_Lean_Data_Lsp_Extra_0__Lean_Lsp_reprLineRa
 _start:
 {
 lean_object* x_1; 
-x_1 = lean_mk_string("{ ");
+x_1 = lean_mk_string_from_bytes("{ ", 2);
 return x_1;
 }
 }
@@ -4292,7 +4291,7 @@ static lean_object* _init_l___private_Lean_Data_Lsp_Extra_0__Lean_Lsp_reprLineRa
 _start:
 {
 lean_object* x_1; 
-x_1 = lean_mk_string(" }");
+x_1 = lean_mk_string_from_bytes(" }", 2);
 return x_1;
 }
 }
