git/leanprover/lean4/stage0/stdlib/Lean/Server/FileWorker/RequestHandling.c
@@ -40,7 +40,7 @@ LEAN_EXPORT lean_object* l_Lean_Server_FileWorker_handleSemanticTokens___lambda_
 LEAN_EXPORT lean_object* l_Lean_Server_FileWorker_handleHover___lambda__2(lean_object*, lean_object*, lean_object*, lean_object*, lean_object*, lean_object*);
 LEAN_EXPORT lean_object* l_Lean_Server_registerLspRequestHandler___at_Lean_Server_FileWorker_initFn____x40_Lean_Server_FileWorker_RequestHandling___hyg_9601____spec__24___lambda__1(lean_object*);
 static lean_object* l_Lean_Server_FileWorker_initFn____x40_Lean_Server_FileWorker_RequestHandling___hyg_9601____closed__14;
-lean_object* l___private_Lean_Data_Lsp_Basic_0__Lean_Lsp_fromJsonTextDocumentPositionParams____x40_Lean_Data_Lsp_Basic___hyg_1983_(lean_object*);
+lean_object* l___private_Lean_Data_Lsp_Basic_0__Lean_Lsp_fromJsonTextDocumentPositionParams____x40_Lean_Data_Lsp_Basic___hyg_1974_(lean_object*);
 extern lean_object* l_Lean_nullKind;
 LEAN_EXPORT uint8_t l_Lean_Server_FileWorker_getInteractiveGoals___lambda__1(lean_object*, lean_object*);
 LEAN_EXPORT lean_object* l_Lean_Server_registerLspRequestHandler___at_Lean_Server_FileWorker_initFn____x40_Lean_Server_FileWorker_RequestHandling___hyg_9601____spec__24(lean_object*, lean_object*, lean_object*);
@@ -65,7 +65,7 @@ LEAN_EXPORT lean_object* l_Lean_Server_registerLspRequestHandler___at_Lean_Serve
 lean_object* lean_io_error_to_string(lean_object*);
 LEAN_EXPORT lean_object* l_Lean_Server_FileWorker_getInteractiveTermGoal___lambda__1(lean_object*, lean_object*, lean_object*, lean_object*, lean_object*, lean_object*, lean_object*);
 LEAN_EXPORT lean_object* l_Lean_Server_registerLspRequestHandler___at_Lean_Server_FileWorker_initFn____x40_Lean_Server_FileWorker_RequestHandling___hyg_9601____spec__14___lambda__2(lean_object*);
-lean_object* l___private_Lean_Data_Lsp_LanguageFeatures_0__Lean_Lsp_fromJsonHoverParams____x40_Lean_Data_Lsp_LanguageFeatures___hyg_1780_(lean_object*);
+lean_object* l___private_Lean_Data_Lsp_LanguageFeatures_0__Lean_Lsp_fromJsonHoverParams____x40_Lean_Data_Lsp_LanguageFeatures___hyg_1759_(lean_object*);
 static lean_object* l_Lean_Server_FileWorker_handleDocumentSymbol_toDocumentSymbols___lambda__3___closed__7;
 lean_object* l___private_Lean_Data_Lsp_Extra_0__Lean_Lsp_fromJsonPlainGoalParams____x40_Lean_Data_Lsp_Extra___hyg_482_(lean_object*);
 lean_object* l_Array_append___rarg(lean_object*, lean_object*);
@@ -217,7 +217,7 @@ static lean_object* l_Lean_Server_registerLspRequestHandler___at_Lean_Server_Fil
 LEAN_EXPORT lean_object* l_Lean_Server_FileWorker_handleDocumentHighlight(lean_object*, lean_object*, lean_object*);
 LEAN_EXPORT lean_object* l_List_forIn_loop___at_Lean_Server_FileWorker_handleSemanticTokens_highlightId___spec__1___lambda__1___boxed(lean_object*, lean_object*, lean_object*, lean_object*, lean_object*, lean_object*, lean_object*, lean_object*, lean_object*);
 lean_object* l_Except_map___rarg(lean_object*, lean_object*);
-lean_object* l___private_Lean_Data_Lsp_LanguageFeatures_0__Lean_Lsp_toJsonHover____x40_Lean_Data_Lsp_LanguageFeatures___hyg_1681_(lean_object*);
+lean_object* l___private_Lean_Data_Lsp_LanguageFeatures_0__Lean_Lsp_toJsonHover____x40_Lean_Data_Lsp_LanguageFeatures___hyg_1663_(lean_object*);
 lean_object* l___private_Lean_Data_Lsp_Extra_0__Lean_Lsp_fromJsonWaitForDiagnosticsParams____x40_Lean_Data_Lsp_Extra___hyg_24_(lean_object*);
 static lean_object* l_Lean_Server_FileWorker_handleDocumentSymbol_toDocumentSymbols___closed__3;
 static lean_object* l_Lean_Server_FileWorker_handleFoldingRange_addCommandRange___closed__1;
@@ -262,7 +262,7 @@ static lean_object* l_Lean_Server_FileWorker_handleDocumentSymbol_toDocumentSymb
 LEAN_EXPORT lean_object* l_Array_forInUnsafe_loop___at_Lean_Server_FileWorker_handleDocumentHighlight___spec__2(lean_object*, lean_object*, size_t, size_t, lean_object*);
 LEAN_EXPORT lean_object* l_Lean_Server_registerLspRequestHandler___at_Lean_Server_FileWorker_initFn____x40_Lean_Server_FileWorker_RequestHandling___hyg_9601____spec__14___lambda__4(lean_object*, lean_object*, lean_object*, lean_object*);
 static lean_object* l_Lean_Server_FileWorker_initFn____x40_Lean_Server_FileWorker_RequestHandling___hyg_9601____closed__3;
-lean_object* l___private_Lean_Data_Lsp_LanguageFeatures_0__Lean_Lsp_toJsonSemanticTokens____x40_Lean_Data_Lsp_LanguageFeatures___hyg_3722_(lean_object*);
+lean_object* l___private_Lean_Data_Lsp_LanguageFeatures_0__Lean_Lsp_toJsonSemanticTokens____x40_Lean_Data_Lsp_LanguageFeatures___hyg_3689_(lean_object*);
 LEAN_EXPORT lean_object* l_Lean_Server_FileWorker_handleFoldingRange_addCommandRange___lambda__1___boxed(lean_object*, lean_object*, lean_object*, lean_object*, lean_object*, lean_object*);
 lean_object* l_Lean_Name_toString(lean_object*, uint8_t);
 LEAN_EXPORT lean_object* l_Array_mapMUnsafe_map___at_Lean_Server_FileWorker_handlePlainGoal___spec__2(size_t, size_t, lean_object*);
@@ -273,7 +273,7 @@ LEAN_EXPORT lean_object* l_Array_mapMUnsafe_map___at_Lean_Server_FileWorker_hand
 LEAN_EXPORT lean_object* l_Lean_Server_registerLspRequestHandler___at_Lean_Server_FileWorker_initFn____x40_Lean_Server_FileWorker_RequestHandling___hyg_9601____spec__27___lambda__5(lean_object*, lean_object*, lean_object*, lean_object*);
 lean_object* l_Std_PersistentHashMap_insert___at_Lean_Server_registerLspRequestHandler___spec__2(lean_object*, lean_object*, lean_object*);
 lean_object* l_Lean_Widget_InteractiveTermGoal_toInteractiveGoal(lean_object*);
-lean_object* l___private_Lean_Data_Lsp_LanguageFeatures_0__Lean_Lsp_fromJsonFoldingRangeParams____x40_Lean_Data_Lsp_LanguageFeatures___hyg_3762_(lean_object*);
+lean_object* l___private_Lean_Data_Lsp_LanguageFeatures_0__Lean_Lsp_fromJsonFoldingRangeParams____x40_Lean_Data_Lsp_LanguageFeatures___hyg_3729_(lean_object*);
 lean_object* l_Lean_Elab_InfoTree_termGoalAt_x3f(lean_object*, lean_object*);
 LEAN_EXPORT lean_object* l_Lean_Server_registerLspRequestHandler___at_Lean_Server_FileWorker_initFn____x40_Lean_Server_FileWorker_RequestHandling___hyg_9601____spec__27___lambda__3(lean_object*, lean_object*, lean_object*, lean_object*);
 lean_object* l_IO_AsyncList_waitAll___rarg(lean_object*, lean_object*, lean_object*);
@@ -286,7 +286,7 @@ LEAN_EXPORT lean_object* l_Lean_Server_FileWorker_handleSemanticTokens_highlight
 LEAN_EXPORT lean_object* l_Lean_Server_FileWorker_handleDocumentHighlight___lambda__3(lean_object*, lean_object*, lean_object*, lean_object*, lean_object*, lean_object*, lean_object*, lean_object*);
 static lean_object* l_Lean_Server_FileWorker_handleSemanticTokensFull___rarg___closed__1;
 static lean_object* l_Lean_Server_registerLspRequestHandler___at_Lean_Server_FileWorker_initFn____x40_Lean_Server_FileWorker_RequestHandling___hyg_9601____spec__7___lambda__3___closed__1;
-lean_object* l___private_Lean_Data_Lsp_LanguageFeatures_0__Lean_Lsp_fromJsonSemanticTokensRangeParams____x40_Lean_Data_Lsp_LanguageFeatures___hyg_3583_(lean_object*);
+lean_object* l___private_Lean_Data_Lsp_LanguageFeatures_0__Lean_Lsp_fromJsonSemanticTokensRangeParams____x40_Lean_Data_Lsp_LanguageFeatures___hyg_3550_(lean_object*);
 LEAN_EXPORT lean_object* l_Lean_Server_FileWorker_handleSemanticTokensFull(lean_object*);
 LEAN_EXPORT lean_object* l_Lean_Server_FileWorker_handleSemanticTokens_highlightId___lambda__1___boxed(lean_object*, lean_object*, lean_object*, lean_object*);
 static lean_object* l_Lean_Server_registerLspRequestHandler___at_Lean_Server_FileWorker_initFn____x40_Lean_Server_FileWorker_RequestHandling___hyg_9601____spec__10___lambda__4___closed__1;
@@ -326,7 +326,7 @@ LEAN_EXPORT lean_object* l_Lean_Server_registerLspRequestHandler___at_Lean_Serve
 LEAN_EXPORT lean_object* l_Array_mapMUnsafe_map___at_Lean_Server_FileWorker_handlePlainGoal___spec__2___boxed(lean_object*, lean_object*, lean_object*);
 lean_object* lean_array_to_list(lean_object*, lean_object*);
 static lean_object* l_Lean_Server_FileWorker_handleDocumentSymbol_toDocumentSymbols___lambda__3___closed__3;
-lean_object* l___private_Lean_Data_Lsp_LanguageFeatures_0__Lean_Lsp_fromJsonSemanticTokensParams____x40_Lean_Data_Lsp_LanguageFeatures___hyg_3500_(lean_object*);
+lean_object* l___private_Lean_Data_Lsp_LanguageFeatures_0__Lean_Lsp_fromJsonSemanticTokensParams____x40_Lean_Data_Lsp_LanguageFeatures___hyg_3467_(lean_object*);
 LEAN_EXPORT lean_object* l_Lean_Server_FileWorker_handlePlainGoal(lean_object*, lean_object*, lean_object*);
 uint8_t l_Lean_Environment_contains(lean_object*, lean_object*);
 LEAN_EXPORT lean_object* l_Lean_Server_FileWorker_handleDefinition___lambda__1___boxed(lean_object*, lean_object*, lean_object*, lean_object*, lean_object*, lean_object*, lean_object*);
@@ -341,11 +341,11 @@ static lean_object* l_Array_mapMUnsafe_map___at_Lean_Server_FileWorker_handlePla
 LEAN_EXPORT lean_object* l_Lean_Server_FileWorker_handleCompletion(lean_object*, lean_object*, lean_object*);
 static lean_object* l_Lean_Server_FileWorker_initFn____x40_Lean_Server_FileWorker_RequestHandling___hyg_9601____closed__11;
 lean_object* l___private_Lean_Data_Lsp_Extra_0__Lean_Lsp_toJsonPlainGoal____x40_Lean_Data_Lsp_Extra___hyg_646_(lean_object*);
-lean_object* l___private_Lean_Data_Lsp_LanguageFeatures_0__Lean_Lsp_fromJsonDocumentSymbolParams____x40_Lean_Data_Lsp_LanguageFeatures___hyg_2668_(lean_object*);
+lean_object* l___private_Lean_Data_Lsp_LanguageFeatures_0__Lean_Lsp_fromJsonDocumentSymbolParams____x40_Lean_Data_Lsp_LanguageFeatures___hyg_2644_(lean_object*);
 LEAN_EXPORT lean_object* l_liftExcept___at_Lean_Server_FileWorker_initFn____x40_Lean_Server_FileWorker_RequestHandling___hyg_9601____spec__26(lean_object*, lean_object*, lean_object*);
 static lean_object* l_Lean_Server_registerLspRequestHandler___at_Lean_Server_FileWorker_initFn____x40_Lean_Server_FileWorker_RequestHandling___hyg_9601____spec__1___lambda__2___closed__1;
 LEAN_EXPORT lean_object* l_Lean_Server_FileWorker_getInteractiveTermGoal___lambda__3___boxed(lean_object*, lean_object*, lean_object*, lean_object*, lean_object*, lean_object*, lean_object*);
-lean_object* l___private_Lean_Data_Lsp_LanguageFeatures_0__Lean_Lsp_toJsonDocumentHighlight____x40_Lean_Data_Lsp_LanguageFeatures___hyg_2617_(lean_object*);
+lean_object* l___private_Lean_Data_Lsp_LanguageFeatures_0__Lean_Lsp_toJsonDocumentHighlight____x40_Lean_Data_Lsp_LanguageFeatures___hyg_2596_(lean_object*);
 lean_object* lean_local_ctx_pop(lean_object*);
 static lean_object* l_Lean_Server_registerLspRequestHandler___at_Lean_Server_FileWorker_initFn____x40_Lean_Server_FileWorker_RequestHandling___hyg_9601____spec__1___lambda__4___closed__2;
 LEAN_EXPORT lean_object* l_Lean_Server_registerLspRequestHandler___at_Lean_Server_FileWorker_initFn____x40_Lean_Server_FileWorker_RequestHandling___hyg_9601____spec__27___lambda__2(lean_object*);
@@ -369,7 +369,7 @@ LEAN_EXPORT lean_object* l_Array_forInUnsafe_loop___at_Lean_Server_FileWorker_ha
 LEAN_EXPORT lean_object* l_Lean_Server_FileWorker_handleDefinition___lambda__12___boxed(lean_object*, lean_object*, lean_object*, lean_object*, lean_object*, lean_object*, lean_object*, lean_object*, lean_object*, lean_object*, lean_object*, lean_object*, lean_object*);
 LEAN_EXPORT lean_object* l_Lean_Server_registerLspRequestHandler___at_Lean_Server_FileWorker_initFn____x40_Lean_Server_FileWorker_RequestHandling___hyg_9601____spec__7___lambda__1(lean_object*);
 static lean_object* l_Lean_Server_FileWorker_handleDocumentSymbol_toDocumentSymbols___lambda__3___closed__9;
-lean_object* l___private_Lean_Data_Lsp_LanguageFeatures_0__Lean_Lsp_fromJsonCompletionParams____x40_Lean_Data_Lsp_LanguageFeatures___hyg_1568_(lean_object*);
+lean_object* l___private_Lean_Data_Lsp_LanguageFeatures_0__Lean_Lsp_fromJsonCompletionParams____x40_Lean_Data_Lsp_LanguageFeatures___hyg_1550_(lean_object*);
 extern lean_object* l_Task_Priority_default;
 LEAN_EXPORT lean_object* l_Lean_Server_registerLspRequestHandler___at_Lean_Server_FileWorker_initFn____x40_Lean_Server_FileWorker_RequestHandling___hyg_9601____spec__18___lambda__1(lean_object*);
 LEAN_EXPORT lean_object* l_Lean_Server_FileWorker_GoToKind_toCtorIdx(uint8_t);
@@ -393,7 +393,7 @@ uint8_t l_Char_isAlpha(uint32_t);
 LEAN_EXPORT lean_object* l_Lean_Server_FileWorker_getInteractiveTermGoal___lambda__2(lean_object*, lean_object*, lean_object*, lean_object*, lean_object*, lean_object*);
 LEAN_EXPORT lean_object* l_Lean_Server_FileWorker_handleDocumentSymbol_toDocumentSymbols___lambda__6(lean_object*, lean_object*, lean_object*, lean_object*, lean_object*, lean_object*, lean_object*, lean_object*);
 static lean_object* l_Lean_Server_FileWorker_noHighlightKinds___closed__5;
-lean_object* l___private_Lean_Data_Lsp_LanguageFeatures_0__Lean_Lsp_toJsonCompletionList____x40_Lean_Data_Lsp_LanguageFeatures___hyg_1517_(lean_object*);
+lean_object* l___private_Lean_Data_Lsp_LanguageFeatures_0__Lean_Lsp_toJsonCompletionList____x40_Lean_Data_Lsp_LanguageFeatures___hyg_1499_(lean_object*);
 static lean_object* l_Lean_Server_FileWorker_initFn____x40_Lean_Server_FileWorker_RequestHandling___hyg_9601____closed__12;
 static lean_object* l_Lean_Server_FileWorker_handleDocumentSymbol_toDocumentSymbols___lambda__3___closed__4;
 static lean_object* l_Lean_Server_registerLspRequestHandler___at_Lean_Server_FileWorker_initFn____x40_Lean_Server_FileWorker_RequestHandling___hyg_9601____spec__1___lambda__5___closed__2;
@@ -414,7 +414,6 @@ static lean_object* l_Lean_Server_FileWorker_noHighlightKinds___closed__14;
 LEAN_EXPORT lean_object* l_Lean_Server_registerLspRequestHandler___at_Lean_Server_FileWorker_initFn____x40_Lean_Server_FileWorker_RequestHandling___hyg_9601____spec__27___lambda__1(lean_object*);
 static lean_object* l_Lean_Server_registerLspRequestHandler___at_Lean_Server_FileWorker_initFn____x40_Lean_Server_FileWorker_RequestHandling___hyg_9601____spec__31___lambda__3___closed__1;
 static lean_object* l_Lean_Server_FileWorker_handlePlainGoal___closed__3;
-LEAN_EXPORT lean_object* l_Lean_Server_registerLspRequestHandler___at_Lean_Server_FileWorker_initFn____x40_Lean_Server_FileWorker_RequestHandling___hyg_9601____spec__7___lambda__2___boxed(lean_object*);
 lean_object* l_Lean_isRec___at___private_Lean_Meta_DiscrTree_0__Lean_Meta_DiscrTree_getKeyArgs___spec__1(lean_object*, lean_object*, lean_object*, lean_object*, lean_object*, lean_object*);
 lean_object* l_Lean_Syntax_getPos_x3f(lean_object*, uint8_t);
 LEAN_EXPORT lean_object* l_Lean_Server_registerLspRequestHandler___at_Lean_Server_FileWorker_initFn____x40_Lean_Server_FileWorker_RequestHandling___hyg_9601____spec__1(lean_object*, lean_object*, lean_object*);
@@ -592,7 +591,7 @@ LEAN_EXPORT lean_object* l_List_spanAux___at_Lean_Server_FileWorker_handleFoldin
 LEAN_EXPORT lean_object* l_Lean_Server_parseRequestParams___at_Lean_Server_FileWorker_initFn____x40_Lean_Server_FileWorker_RequestHandling___hyg_9601____spec__15(lean_object*);
 static lean_object* l_Lean_Server_FileWorker_handleHover___lambda__2___closed__4;
 LEAN_EXPORT uint8_t l_Lean_Server_FileWorker_handleSemanticTokens___lambda__1(lean_object*, lean_object*);
-lean_object* l___private_Lean_Data_Lsp_LanguageFeatures_0__Lean_Lsp_toJsonFoldingRange____x40_Lean_Data_Lsp_LanguageFeatures___hyg_3878_(lean_object*);
+lean_object* l___private_Lean_Data_Lsp_LanguageFeatures_0__Lean_Lsp_toJsonFoldingRange____x40_Lean_Data_Lsp_LanguageFeatures___hyg_3845_(lean_object*);
 static lean_object* l_Lean_Server_FileWorker_handleDocumentHighlight_highlightReturn_x3f___closed__8;
 LEAN_EXPORT lean_object* l_Lean_Server_FileWorker_handleDocumentSymbol___rarg___lambda__2___boxed(lean_object*, lean_object*, lean_object*, lean_object*, lean_object*, lean_object*);
 LEAN_EXPORT lean_object* l_Lean_Server_FileWorker_handleWaitForDiagnostics_waitLoop___boxed(lean_object*, lean_object*, lean_object*);
@@ -657,7 +656,7 @@ LEAN_EXPORT lean_object* l_Lean_Server_FileWorker_handleDocumentHighlight_highli
 LEAN_EXPORT lean_object* l_liftExcept___at_Lean_Server_FileWorker_initFn____x40_Lean_Server_FileWorker_RequestHandling___hyg_9601____spec__6(lean_object*, lean_object*, lean_object*);
 lean_object* l_panic___at_Lean_Elab_InfoTree_smallestInfo_x3f___spec__1(lean_object*);
 uint8_t lean_nat_dec_lt(lean_object*, lean_object*);
-lean_object* l___private_Lean_Data_Lsp_LanguageFeatures_0__Lean_Lsp_fromJsonDocumentHighlightParams____x40_Lean_Data_Lsp_LanguageFeatures___hyg_2481_(lean_object*);
+lean_object* l___private_Lean_Data_Lsp_LanguageFeatures_0__Lean_Lsp_fromJsonDocumentHighlightParams____x40_Lean_Data_Lsp_LanguageFeatures___hyg_2460_(lean_object*);
 static lean_object* l_Lean_Server_FileWorker_initFn____x40_Lean_Server_FileWorker_RequestHandling___hyg_9601____closed__19;
 static lean_object* l_Lean_Server_registerLspRequestHandler___at_Lean_Server_FileWorker_initFn____x40_Lean_Server_FileWorker_RequestHandling___hyg_9601____spec__27___lambda__4___closed__1;
 static lean_object* l_Lean_Server_FileWorker_handlePlainGoal___lambda__1___closed__1;
@@ -930,7 +929,7 @@ static lean_object* _init_l_Lean_Server_FileWorker_handleHover___lambda__2___clo
 _start:
 {
 lean_object* x_1; 
-x_1 = lean_mk_string("Init.Data.Option.BasicAux");
+x_1 = lean_mk_string_from_bytes("Init.Data.Option.BasicAux", 25);
 return x_1;
 }
 }
@@ -938,7 +937,7 @@ static lean_object* _init_l_Lean_Server_FileWorker_handleHover___lambda__2___clo
 _start:
 {
 lean_object* x_1; 
-x_1 = lean_mk_string("Option.get!");
+x_1 = lean_mk_string_from_bytes("Option.get!", 11);
 return x_1;
 }
 }
@@ -946,7 +945,7 @@ static lean_object* _init_l_Lean_Server_FileWorker_handleHover___lambda__2___clo
 _start:
 {
 lean_object* x_1; 
-x_1 = lean_mk_string("value is none");
+x_1 = lean_mk_string_from_bytes("value is none", 13);
 return x_1;
 }
 }
@@ -2579,7 +2578,7 @@ static lean_object* _init_l_Lean_Server_FileWorker_handleDefinition___lambda__2_
 _start:
 {
 lean_object* x_1; 
-x_1 = lean_mk_string("lean");
+x_1 = lean_mk_string_from_bytes("lean", 4);
 return x_1;
 }
 }
@@ -3697,7 +3696,7 @@ static lean_object* _init_l_Lean_Server_FileWorker_handleDefinition___lambda__7_
 _start:
 {
 lean_object* x_1; 
-x_1 = lean_mk_string("import");
+x_1 = lean_mk_string_from_bytes("import", 6);
 return x_1;
 }
 }
@@ -6388,7 +6387,7 @@ static lean_object* _init_l_Array_mapMUnsafe_map___at_Lean_Server_FileWorker_han
 _start:
 {
 lean_object* x_1; 
-x_1 = lean_mk_string("```lean\n");
+x_1 = lean_mk_string_from_bytes("```lean\n", 8);
 return x_1;
 }
 }
@@ -6396,7 +6395,7 @@ static lean_object* _init_l_Array_mapMUnsafe_map___at_Lean_Server_FileWorker_han
 _start:
 {
 lean_object* x_1; 
-x_1 = lean_mk_string("\n```");
+x_1 = lean_mk_string_from_bytes("\n```", 4);
 return x_1;
 }
 }
@@ -6433,7 +6432,7 @@ static lean_object* _init_l_Lean_Server_FileWorker_handlePlainGoal___lambda__1__
 _start:
 {
 lean_object* x_1; 
-x_1 = lean_mk_string("\n---\n");
+x_1 = lean_mk_string_from_bytes("\n---\n", 5);
 return x_1;
 }
 }
@@ -6441,7 +6440,7 @@ static lean_object* _init_l_Lean_Server_FileWorker_handlePlainGoal___lambda__1__
 _start:
 {
 lean_object* x_1; 
-x_1 = lean_mk_string("no goals");
+x_1 = lean_mk_string_from_bytes("no goals", 8);
 return x_1;
 }
 }
@@ -7779,7 +7778,7 @@ static lean_object* _init_l_Lean_Server_FileWorker_handleDocumentHighlight_highl
 _start:
 {
 lean_object* x_1; 
-x_1 = lean_mk_string("Lean");
+x_1 = lean_mk_string_from_bytes("Lean", 4);
 return x_1;
 }
 }
@@ -7797,7 +7796,7 @@ static lean_object* _init_l_Lean_Server_FileWorker_handleDocumentHighlight_highl
 _start:
 {
 lean_object* x_1; 
-x_1 = lean_mk_string("Parser");
+x_1 = lean_mk_string_from_bytes("Parser", 6);
 return x_1;
 }
 }
@@ -7815,7 +7814,7 @@ static lean_object* _init_l_Lean_Server_FileWorker_handleDocumentHighlight_highl
 _start:
 {
 lean_object* x_1; 
-x_1 = lean_mk_string("Term");
+x_1 = lean_mk_string_from_bytes("Term", 4);
 return x_1;
 }
 }
@@ -7833,7 +7832,7 @@ static lean_object* _init_l_Lean_Server_FileWorker_handleDocumentHighlight_highl
 _start:
 {
 lean_object* x_1; 
-x_1 = lean_mk_string("doReturn");
+x_1 = lean_mk_string_from_bytes("doReturn", 8);
 return x_1;
 }
 }
@@ -7851,7 +7850,7 @@ static lean_object* _init_l_Lean_Server_FileWorker_handleDocumentHighlight_highl
 _start:
 {
 lean_object* x_1; 
-x_1 = lean_mk_string("do");
+x_1 = lean_mk_string_from_bytes("do", 2);
 return x_1;
 }
 }
@@ -8707,7 +8706,7 @@ static lean_object* _init_l_Lean_Server_FileWorker_handleDocumentSymbol_toDocume
 _start:
 {
 lean_object* x_1; 
-x_1 = lean_mk_string("declSig");
+x_1 = lean_mk_string_from_bytes("declSig", 7);
 return x_1;
 }
 }
@@ -8715,7 +8714,7 @@ static lean_object* _init_l_Lean_Server_FileWorker_handleDocumentSymbol_toDocume
 _start:
 {
 lean_object* x_1; 
-x_1 = lean_mk_string("declId");
+x_1 = lean_mk_string_from_bytes("declId", 6);
 return x_1;
 }
 }
@@ -8723,7 +8722,7 @@ static lean_object* _init_l_Lean_Server_FileWorker_handleDocumentSymbol_toDocume
 _start:
 {
 lean_object* x_1; 
-x_1 = lean_mk_string("<unknown>");
+x_1 = lean_mk_string_from_bytes("<unknown>", 9);
 return x_1;
 }
 }
@@ -8731,7 +8730,7 @@ static lean_object* _init_l_Lean_Server_FileWorker_handleDocumentSymbol_toDocume
 _start:
 {
 lean_object* x_1; 
-x_1 = lean_mk_string("ident");
+x_1 = lean_mk_string_from_bytes("ident", 5);
 return x_1;
 }
 }
@@ -8749,7 +8748,7 @@ static lean_object* _init_l_Lean_Server_FileWorker_handleDocumentSymbol_toDocume
 _start:
 {
 lean_object* x_1; 
-x_1 = lean_mk_string("instance ");
+x_1 = lean_mk_string_from_bytes("instance ", 9);
 return x_1;
 }
 }
@@ -8757,7 +8756,7 @@ static lean_object* _init_l_Lean_Server_FileWorker_handleDocumentSymbol_toDocume
 _start:
 {
 lean_object* x_1; 
-x_1 = lean_mk_string("");
+x_1 = lean_mk_string_from_bytes("", 0);
 return x_1;
 }
 }
@@ -10000,7 +9999,7 @@ static lean_object* _init_l_Lean_Server_FileWorker_handleDocumentSymbol_toDocume
 _start:
 {
 lean_object* x_1; 
-x_1 = lean_mk_string("declaration");
+x_1 = lean_mk_string_from_bytes("declaration", 11);
 return x_1;
 }
 }
@@ -10008,7 +10007,7 @@ static lean_object* _init_l_Lean_Server_FileWorker_handleDocumentSymbol_toDocume
 _start:
 {
 lean_object* x_1; 
-x_1 = lean_mk_string("declModifiers");
+x_1 = lean_mk_string_from_bytes("declModifiers", 13);
 return x_1;
 }
 }
@@ -10016,7 +10015,7 @@ static lean_object* _init_l_Lean_Server_FileWorker_handleDocumentSymbol_toDocume
 _start:
 {
 lean_object* x_1; 
-x_1 = lean_mk_string("instance");
+x_1 = lean_mk_string_from_bytes("instance", 8);
 return x_1;
 }
 }
@@ -10024,7 +10023,7 @@ static lean_object* _init_l_Lean_Server_FileWorker_handleDocumentSymbol_toDocume
 _start:
 {
 lean_object* x_1; 
-x_1 = lean_mk_string("attrKind");
+x_1 = lean_mk_string_from_bytes("attrKind", 8);
 return x_1;
 }
 }
@@ -10032,7 +10031,7 @@ static lean_object* _init_l_Lean_Server_FileWorker_handleDocumentSymbol_toDocume
 _start:
 {
 lean_object* x_1; 
-x_1 = lean_mk_string("namedPrio");
+x_1 = lean_mk_string_from_bytes("namedPrio", 9);
 return x_1;
 }
 }
@@ -12267,7 +12266,7 @@ static lean_object* _init_l_Lean_Server_FileWorker_handleDocumentSymbol_toDocume
 _start:
 {
 lean_object* x_1; 
-x_1 = lean_mk_string("Command");
+x_1 = lean_mk_string_from_bytes("Command", 7);
 return x_1;
 }
 }
@@ -12285,7 +12284,7 @@ static lean_object* _init_l_Lean_Server_FileWorker_handleDocumentSymbol_toDocume
 _start:
 {
 lean_object* x_1; 
-x_1 = lean_mk_string("namespace");
+x_1 = lean_mk_string_from_bytes("namespace", 9);
 return x_1;
 }
 }
@@ -12303,7 +12302,7 @@ static lean_object* _init_l_Lean_Server_FileWorker_handleDocumentSymbol_toDocume
 _start:
 {
 lean_object* x_1; 
-x_1 = lean_mk_string("section");
+x_1 = lean_mk_string_from_bytes("section", 7);
 return x_1;
 }
 }
@@ -12321,7 +12320,7 @@ static lean_object* _init_l_Lean_Server_FileWorker_handleDocumentSymbol_toDocume
 _start:
 {
 lean_object* x_1; 
-x_1 = lean_mk_string("end");
+x_1 = lean_mk_string_from_bytes("end", 3);
 return x_1;
 }
 }
@@ -12349,7 +12348,7 @@ static lean_object* _init_l_Lean_Server_FileWorker_handleDocumentSymbol_toDocume
 _start:
 {
 lean_object* x_1; 
-x_1 = lean_mk_string("<section>");
+x_1 = lean_mk_string_from_bytes("<section>", 9);
 return x_1;
 }
 }
@@ -13227,7 +13226,7 @@ static lean_object* _init_l_Lean_Server_FileWorker_noHighlightKinds___closed__1(
 _start:
 {
 lean_object* x_1; 
-x_1 = lean_mk_string("sorry");
+x_1 = lean_mk_string_from_bytes("sorry", 5);
 return x_1;
 }
 }
@@ -13245,7 +13244,7 @@ static lean_object* _init_l_Lean_Server_FileWorker_noHighlightKinds___closed__3(
 _start:
 {
 lean_object* x_1; 
-x_1 = lean_mk_string("type");
+x_1 = lean_mk_string_from_bytes("type", 4);
 return x_1;
 }
 }
@@ -13263,7 +13262,7 @@ static lean_object* _init_l_Lean_Server_FileWorker_noHighlightKinds___closed__5(
 _start:
 {
 lean_object* x_1; 
-x_1 = lean_mk_string("prop");
+x_1 = lean_mk_string_from_bytes("prop", 4);
 return x_1;
 }
 }
@@ -13281,7 +13280,7 @@ static lean_object* _init_l_Lean_Server_FileWorker_noHighlightKinds___closed__7(
 _start:
 {
 lean_object* x_1; 
-x_1 = lean_mk_string("antiquotName");
+x_1 = lean_mk_string_from_bytes("antiquotName", 12);
 return x_1;
 }
 }
@@ -13299,7 +13298,7 @@ static lean_object* _init_l_Lean_Server_FileWorker_noHighlightKinds___closed__9(
 _start:
 {
 lean_object* x_1; 
-x_1 = lean_mk_string("docComment");
+x_1 = lean_mk_string_from_bytes("docComment", 10);
 return x_1;
 }
 }
@@ -14409,7 +14408,7 @@ static lean_object* _init_l_Lean_Server_FileWorker_handleSemanticTokens_go___clo
 _start:
 {
 lean_object* x_1; 
-x_1 = lean_mk_string("proj");
+x_1 = lean_mk_string_from_bytes("proj", 4);
 return x_1;
 }
 }
@@ -15432,7 +15431,7 @@ static lean_object* _init_l_Lean_Server_FileWorker_handleFoldingRange_isImport__
 _start:
 {
 lean_object* x_1; 
-x_1 = lean_mk_string("Module");
+x_1 = lean_mk_string_from_bytes("Module", 6);
 return x_1;
 }
 }
@@ -15450,7 +15449,7 @@ static lean_object* _init_l_Lean_Server_FileWorker_handleFoldingRange_isImport__
 _start:
 {
 lean_object* x_1; 
-x_1 = lean_mk_string("header");
+x_1 = lean_mk_string_from_bytes("header", 6);
 return x_1;
 }
 }
@@ -15468,7 +15467,7 @@ static lean_object* _init_l_Lean_Server_FileWorker_handleFoldingRange_isImport__
 _start:
 {
 lean_object* x_1; 
-x_1 = lean_mk_string("open");
+x_1 = lean_mk_string_from_bytes("open", 4);
 return x_1;
 }
 }
@@ -15704,7 +15703,7 @@ static lean_object* _init_l_Lean_Server_FileWorker_handleFoldingRange_addCommand
 _start:
 {
 lean_object* x_1; 
-x_1 = lean_mk_string("moduleDoc");
+x_1 = lean_mk_string_from_bytes("moduleDoc", 9);
 return x_1;
 }
 }
@@ -16063,7 +16062,7 @@ static lean_object* _init_l_Lean_Server_FileWorker_handleFoldingRange_addRanges_
 _start:
 {
 lean_object* x_1; 
-x_1 = lean_mk_string("mutual");
+x_1 = lean_mk_string_from_bytes("mutual", 6);
 return x_1;
 }
 }
@@ -17179,7 +17178,7 @@ static lean_object* _init_l_Lean_Server_parseRequestParams___at_Lean_Server_File
 _start:
 {
 lean_object* x_1; 
-x_1 = lean_mk_string("Cannot parse request params: ");
+x_1 = lean_mk_string_from_bytes("Cannot parse request params: ", 29);
 return x_1;
 }
 }
@@ -17187,7 +17186,7 @@ static lean_object* _init_l_Lean_Server_parseRequestParams___at_Lean_Server_File
 _start:
 {
 lean_object* x_1; 
-x_1 = lean_mk_string("\n");
+x_1 = lean_mk_string_from_bytes("\n", 1);
 return x_1;
 }
 }
@@ -17537,7 +17536,7 @@ static lean_object* _init_l_Lean_Server_registerLspRequestHandler___at_Lean_Serv
 _start:
 {
 lean_object* x_1; 
-x_1 = lean_mk_string("Failed to register LSP request handler for '");
+x_1 = lean_mk_string_from_bytes("Failed to register LSP request handler for '", 44);
 return x_1;
 }
 }
@@ -17545,7 +17544,7 @@ static lean_object* _init_l_Lean_Server_registerLspRequestHandler___at_Lean_Serv
 _start:
 {
 lean_object* x_1; 
-x_1 = lean_mk_string("': already registered");
+x_1 = lean_mk_string_from_bytes("': already registered", 21);
 return x_1;
 }
 }
@@ -17628,7 +17627,7 @@ static lean_object* _init_l_Lean_Server_registerLspRequestHandler___at_Lean_Serv
 _start:
 {
 lean_object* x_1; 
-x_1 = lean_mk_string("': only possible during initialization");
+x_1 = lean_mk_string_from_bytes("': only possible during initialization", 38);
 return x_1;
 }
 }
@@ -17697,7 +17696,7 @@ LEAN_EXPORT lean_object* l_Lean_Server_parseRequestParams___at_Lean_Server_FileW
 _start:
 {
 lean_object* x_2; 
-x_2 = l___private_Lean_Data_Lsp_LanguageFeatures_0__Lean_Lsp_fromJsonCompletionParams____x40_Lean_Data_Lsp_LanguageFeatures___hyg_1568_(x_1);
+x_2 = l___private_Lean_Data_Lsp_LanguageFeatures_0__Lean_Lsp_fromJsonCompletionParams____x40_Lean_Data_Lsp_LanguageFeatures___hyg_1550_(x_1);
 if (lean_obj_tag(x_2) == 0)
 {
 uint8_t x_3; 
@@ -17853,7 +17852,7 @@ static lean_object* _init_l_Lean_Server_registerLspRequestHandler___at_Lean_Serv
 _start:
 {
 lean_object* x_1; 
-x_1 = lean_alloc_closure((void*)(l___private_Lean_Data_Lsp_LanguageFeatures_0__Lean_Lsp_toJsonCompletionList____x40_Lean_Data_Lsp_LanguageFeatures___hyg_1517_), 1, 0);
+x_1 = lean_alloc_closure((void*)(l___private_Lean_Data_Lsp_LanguageFeatures_0__Lean_Lsp_toJsonCompletionList____x40_Lean_Data_Lsp_LanguageFeatures___hyg_1499_), 1, 0);
 return x_1;
 }
 }
@@ -18150,7 +18149,7 @@ LEAN_EXPORT lean_object* l_Lean_Server_parseRequestParams___at_Lean_Server_FileW
 _start:
 {
 lean_object* x_2; 
-x_2 = l___private_Lean_Data_Lsp_LanguageFeatures_0__Lean_Lsp_fromJsonHoverParams____x40_Lean_Data_Lsp_LanguageFeatures___hyg_1780_(x_1);
+x_2 = l___private_Lean_Data_Lsp_LanguageFeatures_0__Lean_Lsp_fromJsonHoverParams____x40_Lean_Data_Lsp_LanguageFeatures___hyg_1759_(x_1);
 if (lean_obj_tag(x_2) == 0)
 {
 uint8_t x_3; 
@@ -18315,7 +18314,9 @@ else
 {
 lean_object* x_3; lean_object* x_4; 
 x_3 = lean_ctor_get(x_1, 0);
-x_4 = l___private_Lean_Data_Lsp_LanguageFeatures_0__Lean_Lsp_toJsonHover____x40_Lean_Data_Lsp_LanguageFeatures___hyg_1681_(x_3);
+lean_inc(x_3);
+lean_dec(x_1);
+x_4 = l___private_Lean_Data_Lsp_LanguageFeatures_0__Lean_Lsp_toJsonHover____x40_Lean_Data_Lsp_LanguageFeatures___hyg_1663_(x_3);
 return x_4;
 }
 }
@@ -18324,7 +18325,7 @@ static lean_object* _init_l_Lean_Server_registerLspRequestHandler___at_Lean_Serv
 _start:
 {
 lean_object* x_1; 
-x_1 = lean_alloc_closure((void*)(l_Lean_Server_registerLspRequestHandler___at_Lean_Server_FileWorker_initFn____x40_Lean_Server_FileWorker_RequestHandling___hyg_9601____spec__7___lambda__2___boxed), 1, 0);
+x_1 = lean_alloc_closure((void*)(l_Lean_Server_registerLspRequestHandler___at_Lean_Server_FileWorker_initFn____x40_Lean_Server_FileWorker_RequestHandling___hyg_9601____spec__7___lambda__2), 1, 0);
 return x_1;
 }
 }
@@ -18621,7 +18622,7 @@ LEAN_EXPORT lean_object* l_Lean_Server_parseRequestParams___at_Lean_Server_FileW
 _start:
 {
 lean_object* x_2; 
-x_2 = l___private_Lean_Data_Lsp_Basic_0__Lean_Lsp_fromJsonTextDocumentPositionParams____x40_Lean_Data_Lsp_Basic___hyg_1983_(x_1);
+x_2 = l___private_Lean_Data_Lsp_Basic_0__Lean_Lsp_fromJsonTextDocumentPositionParams____x40_Lean_Data_Lsp_Basic___hyg_1974_(x_1);
 if (lean_obj_tag(x_2) == 0)
 {
 uint8_t x_3; 
@@ -19113,7 +19114,7 @@ LEAN_EXPORT lean_object* l_Lean_Server_parseRequestParams___at_Lean_Server_FileW
 _start:
 {
 lean_object* x_2; 
-x_2 = l___private_Lean_Data_Lsp_LanguageFeatures_0__Lean_Lsp_fromJsonDocumentHighlightParams____x40_Lean_Data_Lsp_LanguageFeatures___hyg_2481_(x_1);
+x_2 = l___private_Lean_Data_Lsp_LanguageFeatures_0__Lean_Lsp_fromJsonDocumentHighlightParams____x40_Lean_Data_Lsp_LanguageFeatures___hyg_2460_(x_1);
 if (lean_obj_tag(x_2) == 0)
 {
 uint8_t x_3; 
@@ -19226,7 +19227,7 @@ lean_object* x_5; lean_object* x_6; lean_object* x_7; lean_object* x_8; size_t x
 x_5 = lean_array_uget(x_3, x_2);
 x_6 = lean_unsigned_to_nat(0u);
 x_7 = lean_array_uset(x_3, x_2, x_6);
-x_8 = l___private_Lean_Data_Lsp_LanguageFeatures_0__Lean_Lsp_toJsonDocumentHighlight____x40_Lean_Data_Lsp_LanguageFeatures___hyg_2617_(x_5);
+x_8 = l___private_Lean_Data_Lsp_LanguageFeatures_0__Lean_Lsp_toJsonDocumentHighlight____x40_Lean_Data_Lsp_LanguageFeatures___hyg_2596_(x_5);
 x_9 = 1;
 x_10 = lean_usize_add(x_2, x_9);
 x_11 = lean_array_uset(x_7, x_2, x_8);
@@ -19605,7 +19606,7 @@ LEAN_EXPORT lean_object* l_Lean_Server_parseRequestParams___at_Lean_Server_FileW
 _start:
 {
 lean_object* x_2; 
-x_2 = l___private_Lean_Data_Lsp_LanguageFeatures_0__Lean_Lsp_fromJsonDocumentSymbolParams____x40_Lean_Data_Lsp_LanguageFeatures___hyg_2668_(x_1);
+x_2 = l___private_Lean_Data_Lsp_LanguageFeatures_0__Lean_Lsp_fromJsonDocumentSymbolParams____x40_Lean_Data_Lsp_LanguageFeatures___hyg_2644_(x_1);
 if (lean_obj_tag(x_2) == 0)
 {
 uint8_t x_3; 
@@ -20063,7 +20064,7 @@ LEAN_EXPORT lean_object* l_Lean_Server_parseRequestParams___at_Lean_Server_FileW
 _start:
 {
 lean_object* x_2; 
-x_2 = l___private_Lean_Data_Lsp_LanguageFeatures_0__Lean_Lsp_fromJsonSemanticTokensParams____x40_Lean_Data_Lsp_LanguageFeatures___hyg_3500_(x_1);
+x_2 = l___private_Lean_Data_Lsp_LanguageFeatures_0__Lean_Lsp_fromJsonSemanticTokensParams____x40_Lean_Data_Lsp_LanguageFeatures___hyg_3467_(x_1);
 if (lean_obj_tag(x_2) == 0)
 {
 uint8_t x_3; 
@@ -20210,7 +20211,7 @@ static lean_object* _init_l_Lean_Server_registerLspRequestHandler___at_Lean_Serv
 _start:
 {
 lean_object* x_1; 
-x_1 = lean_alloc_closure((void*)(l___private_Lean_Data_Lsp_LanguageFeatures_0__Lean_Lsp_toJsonSemanticTokens____x40_Lean_Data_Lsp_LanguageFeatures___hyg_3722_), 1, 0);
+x_1 = lean_alloc_closure((void*)(l___private_Lean_Data_Lsp_LanguageFeatures_0__Lean_Lsp_toJsonSemanticTokens____x40_Lean_Data_Lsp_LanguageFeatures___hyg_3689_), 1, 0);
 return x_1;
 }
 }
@@ -20507,7 +20508,7 @@ LEAN_EXPORT lean_object* l_Lean_Server_parseRequestParams___at_Lean_Server_FileW
 _start:
 {
 lean_object* x_2; 
-x_2 = l___private_Lean_Data_Lsp_LanguageFeatures_0__Lean_Lsp_fromJsonSemanticTokensRangeParams____x40_Lean_Data_Lsp_LanguageFeatures___hyg_3583_(x_1);
+x_2 = l___private_Lean_Data_Lsp_LanguageFeatures_0__Lean_Lsp_fromJsonSemanticTokensRangeParams____x40_Lean_Data_Lsp_LanguageFeatures___hyg_3550_(x_1);
 if (lean_obj_tag(x_2) == 0)
 {
 uint8_t x_3; 
@@ -20942,7 +20943,7 @@ LEAN_EXPORT lean_object* l_Lean_Server_parseRequestParams___at_Lean_Server_FileW
 _start:
 {
 lean_object* x_2; 
-x_2 = l___private_Lean_Data_Lsp_LanguageFeatures_0__Lean_Lsp_fromJsonFoldingRangeParams____x40_Lean_Data_Lsp_LanguageFeatures___hyg_3762_(x_1);
+x_2 = l___private_Lean_Data_Lsp_LanguageFeatures_0__Lean_Lsp_fromJsonFoldingRangeParams____x40_Lean_Data_Lsp_LanguageFeatures___hyg_3729_(x_1);
 if (lean_obj_tag(x_2) == 0)
 {
 uint8_t x_3; 
@@ -21055,7 +21056,7 @@ lean_object* x_5; lean_object* x_6; lean_object* x_7; lean_object* x_8; size_t x
 x_5 = lean_array_uget(x_3, x_2);
 x_6 = lean_unsigned_to_nat(0u);
 x_7 = lean_array_uset(x_3, x_2, x_6);
-x_8 = l___private_Lean_Data_Lsp_LanguageFeatures_0__Lean_Lsp_toJsonFoldingRange____x40_Lean_Data_Lsp_LanguageFeatures___hyg_3878_(x_5);
+x_8 = l___private_Lean_Data_Lsp_LanguageFeatures_0__Lean_Lsp_toJsonFoldingRange____x40_Lean_Data_Lsp_LanguageFeatures___hyg_3845_(x_5);
 x_9 = 1;
 x_10 = lean_usize_add(x_2, x_9);
 x_11 = lean_array_uset(x_7, x_2, x_8);
@@ -22371,7 +22372,7 @@ static lean_object* _init_l_Lean_Server_FileWorker_initFn____x40_Lean_Server_Fil
 _start:
 {
 lean_object* x_1; 
-x_1 = lean_mk_string("textDocument/waitForDiagnostics");
+x_1 = lean_mk_string_from_bytes("textDocument/waitForDiagnostics", 31);
 return x_1;
 }
 }
@@ -22387,7 +22388,7 @@ static lean_object* _init_l_Lean_Server_FileWorker_initFn____x40_Lean_Server_Fil
 _start:
 {
 lean_object* x_1; 
-x_1 = lean_mk_string("textDocument/completion");
+x_1 = lean_mk_string_from_bytes("textDocument/completion", 23);
 return x_1;
 }
 }
@@ -22403,7 +22404,7 @@ static lean_object* _init_l_Lean_Server_FileWorker_initFn____x40_Lean_Server_Fil
 _start:
 {
 lean_object* x_1; 
-x_1 = lean_mk_string("textDocument/hover");
+x_1 = lean_mk_string_from_bytes("textDocument/hover", 18);
 return x_1;
 }
 }
@@ -22430,7 +22431,7 @@ static lean_object* _init_l_Lean_Server_FileWorker_initFn____x40_Lean_Server_Fil
 _start:
 {
 lean_object* x_1; 
-x_1 = lean_mk_string("textDocument/declaration");
+x_1 = lean_mk_string_from_bytes("textDocument/declaration", 24);
 return x_1;
 }
 }
@@ -22449,7 +22450,7 @@ static lean_object* _init_l_Lean_Server_FileWorker_initFn____x40_Lean_Server_Fil
 _start:
 {
 lean_object* x_1; 
-x_1 = lean_mk_string("textDocument/definition");
+x_1 = lean_mk_string_from_bytes("textDocument/definition", 23);
 return x_1;
 }
 }
@@ -22468,7 +22469,7 @@ static lean_object* _init_l_Lean_Server_FileWorker_initFn____x40_Lean_Server_Fil
 _start:
 {
 lean_object* x_1; 
-x_1 = lean_mk_string("textDocument/typeDefinition");
+x_1 = lean_mk_string_from_bytes("textDocument/typeDefinition", 27);
 return x_1;
 }
 }
@@ -22476,7 +22477,7 @@ static lean_object* _init_l_Lean_Server_FileWorker_initFn____x40_Lean_Server_Fil
 _start:
 {
 lean_object* x_1; 
-x_1 = lean_mk_string("textDocument/documentHighlight");
+x_1 = lean_mk_string_from_bytes("textDocument/documentHighlight", 30);
 return x_1;
 }
 }
@@ -22492,7 +22493,7 @@ static lean_object* _init_l_Lean_Server_FileWorker_initFn____x40_Lean_Server_Fil
 _start:
 {
 lean_object* x_1; 
-x_1 = lean_mk_string("textDocument/documentSymbol");
+x_1 = lean_mk_string_from_bytes("textDocument/documentSymbol", 27);
 return x_1;
 }
 }
@@ -22508,7 +22509,7 @@ static lean_object* _init_l_Lean_Server_FileWorker_initFn____x40_Lean_Server_Fil
 _start:
 {
 lean_object* x_1; 
-x_1 = lean_mk_string("textDocument/semanticTokens/full");
+x_1 = lean_mk_string_from_bytes("textDocument/semanticTokens/full", 32);
 return x_1;
 }
 }
@@ -22524,7 +22525,7 @@ static lean_object* _init_l_Lean_Server_FileWorker_initFn____x40_Lean_Server_Fil
 _start:
 {
 lean_object* x_1; 
-x_1 = lean_mk_string("textDocument/semanticTokens/range");
+x_1 = lean_mk_string_from_bytes("textDocument/semanticTokens/range", 33);
 return x_1;
 }
 }
@@ -22540,7 +22541,7 @@ static lean_object* _init_l_Lean_Server_FileWorker_initFn____x40_Lean_Server_Fil
 _start:
 {
 lean_object* x_1; 
-x_1 = lean_mk_string("textDocument/foldingRange");
+x_1 = lean_mk_string_from_bytes("textDocument/foldingRange", 25);
 return x_1;
 }
 }
@@ -22556,7 +22557,7 @@ static lean_object* _init_l_Lean_Server_FileWorker_initFn____x40_Lean_Server_Fil
 _start:
 {
 lean_object* x_1; 
-x_1 = lean_mk_string("$/lean/plainGoal");
+x_1 = lean_mk_string_from_bytes("$/lean/plainGoal", 16);
 return x_1;
 }
 }
@@ -22572,7 +22573,7 @@ static lean_object* _init_l_Lean_Server_FileWorker_initFn____x40_Lean_Server_Fil
 _start:
 {
 lean_object* x_1; 
-x_1 = lean_mk_string("$/lean/plainTermGoal");
+x_1 = lean_mk_string_from_bytes("$/lean/plainTermGoal", 20);
 return x_1;
 }
 }
@@ -23033,15 +23034,6 @@ x_4 = l_liftExcept___at_Lean_Server_FileWorker_initFn____x40_Lean_Server_FileWor
 lean_dec(x_2);
 lean_dec(x_1);
 return x_4;
-}
-}
-LEAN_EXPORT lean_object* l_Lean_Server_registerLspRequestHandler___at_Lean_Server_FileWorker_initFn____x40_Lean_Server_FileWorker_RequestHandling___hyg_9601____spec__7___lambda__2___boxed(lean_object* x_1) {
-_start:
-{
-lean_object* x_2; 
-x_2 = l_Lean_Server_registerLspRequestHandler___at_Lean_Server_FileWorker_initFn____x40_Lean_Server_FileWorker_RequestHandling___hyg_9601____spec__7___lambda__2(x_1);
-lean_dec(x_1);
-return x_2;
 }
 }
 LEAN_EXPORT lean_object* l_Lean_Server_registerLspRequestHandler___at_Lean_Server_FileWorker_initFn____x40_Lean_Server_FileWorker_RequestHandling___hyg_9601____spec__7___lambda__4___boxed(lean_object* x_1, lean_object* x_2, lean_object* x_3, lean_object* x_4) {
