git/Augustindou/natural2lean-lean-project-template/examples/example-3-contrapositive/theorem.lean
@@ -1,16 +1,61 @@
-import LeanUtils.Div
-import LeanUtils.Logic
-import LeanUtils.Specific
-
+import LeanUtils
 open Nat
 
-theorem square_of_q_divisible_by_3_means_q_is_divisible_by_3 (q : Nat) : divisible 3 (q^2) → divisible 3 q := by 
-  have contrap : ¬(divisible 3 q) → ¬(divisible 3 (q^2)) := by 
-    repeat rw [divisible]
-    intros h₁
-    have h₂ : q^2 % 3 = 1 := by
-      apply square_mod_3 q h₁
+-- first theorem
+theorem square_mod_3 (q : Nat) : (¬divisible 3 q) → (q^2 % 3 = 1) := by
+  intros h₁
+  apply mod_rewrite.mpr
+  have h2 : q % 3 = 0 ∨ q % 3 = 1 ∨ q % 3 = 2 := mod_3_poss _
 
-    simp [*]
+  -- divide cases into 3 goals
+  rcases h2 with h2 | h2 | h2
 
-  exact contrapositive.mpr contrap
+  contradiction
+
+  have ⟨k, h3⟩ : ∃ (k : Nat), q = 3 * k + 1 := by 
+    simp at *
+    assumption
+
+  have q_square : q^2 = 3 * (3 * k^2 + 2 * k) + 1  := by 
+    calc
+      q^2 = (3 * k + 1)^2 := by try simp [*]; try ring
+      _ = 9 * k^2 + 6 * k + 1 := by try simp [*]; try ring
+      _ = 3 * (3 * k^2 + 2 * k) + 1 := by try simp [*]; try ring
+  exact ⟨_, by assumption⟩
+
+  have ⟨k, h3⟩ : ∃ (k : Nat), q = 3 * k + 2 := by 
+    simp at *
+    assumption
+  have q_square : q^2 = 3 * (3 * k^2 + 4 * k + 1) + 1 := by 
+    calc
+      q^2 = (3 * k + 2)^2 := by try simp [*]; try ring
+      _ = 3 * (3 * k^2 + 4 * k + 1) + 1 := by try simp [*]; try ring
+  exact ⟨_, by assumption⟩
+
+-- second using the first
+theorem square_of_q_divisible_by_3_means_q_is_divisible_by_3 (q : Nat) (h₁ : divisible 3 (q^2)) : divisible 3 q := by 
+
+  revert h₁
+  rw [not_imp_not.symm]
+  simp [not_not]
+  intro h₁
+
+  have h₂ : q^2 % 3 = 1 := by
+    try simp_all [square_mod_3]
+    try ring
+  
+  simp_all [divisible]
+
+
+
+  -- have contrap : ¬(divisible 3 q) → ¬(divisible 3 (q^2)) := by 
+  --   intros h₁
+  --   have h₂ : q^2 % 3 = 1 := by
+  --     calc
+  --       q^2 % 3 = 1 := by 
+  --         apply square_mod_3
+  --         try simp [*]; try ring
+    
+  --   simp [*]
+
+  -- exact contrapositive.mpr contrap
