git/arthurpaulino/TestPrettyPrinter/Foo.lean
@@ -1,3 +1,0 @@
-def qq : Bool := true
-
-def foo : List (String × String) := [("asdf", "zxcv")]
