git/larsk21/iris-lean/src/Iris/Proofmode/Theorems.lean
@@ -45,11 +45,11 @@ theorem tac_wand_intro_intuitionistic [BI PROP] {Γₚ Γₛ : List PROP} {P P' 
 
 -- assumptions
 theorem tac_assumption [BI PROP] {Γₚ Γₛ : List PROP} (i : EnvsIndex Γₚ.length Γₛ.length) (Q : PROP) :
-  let (p, i, P) : Bool × Nat × PROP := match i with
-    | .p i => (true, i, Γₚ.getR i)
-    | .s i => (false, i, Γₛ.getR i)
+  let (p, P) : Bool × PROP := match i with
+    | .p i => (true, Γₚ.getR i)
+    | .s i => (false, Γₛ.getR i)
   [FromAssumption p P Q] →
-  let Γₛ' := Γₛ.eraseIdxR i
+  let Γₛ' := if let .s i := i then Γₛ.eraseIdxR i else Γₛ
   [TCIte Γₛ'.isEmptyR TCTrue (TCOr (Absorbing Q) (AffineEnv Γₛ'))] →
   envs_entails ⟨Γₚ, Γₛ⟩ Q
 := sorry
@@ -61,6 +61,23 @@ theorem tac_false_destruct [BI PROP] {Γₚ Γₛ : List PROP} (i : EnvsIndex Γ
     | .s i => Γₛ.getR i
   P = `[iprop| False] →
   envs_entails ⟨Γₚ, Γₛ⟩ Q
+:= sorry
+
+-- (separating) conjunction splitting
+theorem tac_and_split [BI PROP] {Δ : Envs PROP} {Q1 Q2 : PROP} (P : PROP) :
+  [FromAnd P Q1 Q2] →
+  envs_entails Δ Q1 →
+  envs_entails Δ Q2 →
+  envs_entails Δ P
+:= sorry
+
+theorem tac_sep_split [BI PROP] {Γₚ Γₛ : List PROP} {Q1 Q2 : PROP} (sortedIndices : List Nat) (splitRight : Bool) (P : PROP) :
+  [FromSep P Q1 Q2] →
+  let (Γₛ₁, Γₛ₂) := Γₛ.splitWithSortedIndices sortedIndices
+  let (Γₛ₁, Γₛ₂) := if splitRight then (Γₛ₂, Γₛ₁) else (Γₛ₁, Γₛ₂)
+  envs_entails ⟨Γₚ, Γₛ₁⟩ Q1 →
+  envs_entails ⟨Γₚ, Γₛ₂⟩ Q2 →
+  envs_entails ⟨Γₚ, Γₛ⟩ P
 := sorry
 
 end Iris.Proofmode
