git/leanprover/lean4/doc/examples/NFM2022/nfm13.lean
@@ -1,3 +1,4 @@
+/- Type classes are heavily used in Lean -/
 namespace Example
 
 class Mul (α : Type u) where
@@ -5,8 +6,16 @@ class Mul (α : Type u) where
 
 infixl:70 " * " => Mul.mul
 
+def double [Mul α] (a : α) := a * a
+
 class Semigroup (α : Type u) extends Mul α where
   mul_assoc : ∀ a b c : α, (a * b) * c = a * (b * c)
+
+instance : Semigroup Nat where
+  mul := Nat.mul
+  mul_assoc := Nat.mul_assoc
+
+#eval double 5
 
 class Functor (f : Type u → Type v) : Type (max (u+1) v) where
   map : (α → β) → f α → f β
@@ -18,3 +27,18 @@ class LawfulFunctor (f : Type u → Type v) [Functor f] : Prop where
   comp_map (g : α → β) (h : β → γ) (x : f α) :(h ∘ g) <$> x = h <$> g <$> x
 
 end Example
+
+/-
+`Deriving instances automatically`
+
+We have seen `deriving Repr` in a few examples.
+It is an instance generator.
+Lean comes equipped with generators for the following classes.
+`Repr`, `Inhabited`, `BEq`, `DecidableEq`,
+`Hashable`, `Ord`, `FromToJson`, `SizeOf`
+-/
+
+inductive Tree (α : Type u) where
+  | leaf (val : α)
+  | node (left right : Tree α)
+  deriving DecidableEq, Ord, Inhabited, Repr
