git/opencompl/lean-mlir/MLIR/Dialects/ControlFlowSemantics.lean
@@ -1,0 +1,229 @@
+import MLIR.Dialects.ToyModel
+import MLIR.Semantics.Fitree
+import MLIR.Semantics.Verifier
+import MLIR.Semantics.SSAEnv
+import MLIR.Semantics.InvalidOp
+import MLIR.Util.Metagen
+
+import MLIR.AST
+import MLIR.EDSL
+
+import Lean
+
+open MLIR.AST
+
+
+set_option hygiene false in
+genInductive ControlFlowOp #[
+  OpSpec.mk "cf.br" `(
+    (target: String) →
+    (args: List ((τ: MLIRTy) × τ.eval)) →
+    ControlFlowOp Unit)
+  , OpSpec.mk "cf.condbr" `(
+    (cond: Bool)  →
+    ControlFlowOp Unit)
+  -- , OpSpec.mk "runRegion" `(
+  --    (region: Region) →
+  --    (τ: MLIRTy) →
+  --    ControlFlowOp (τ.eval))
+  ]
+
+#check ControlFlowOp
+
+
+-- | What's the return type? x(
+inductive BranchType
+| Br (bbname: BBName)
+| Ret
+
+
+-- | interpret branch and conditional branch
+def cf_semantics_op {E: Type -> Type}: Op → Fitree (InvalidOpE +' SSAEnvE +' E) (Option BranchType)
+  | Op.mk "cf.br" [] [bbname] [] _ _ => do
+        return (BranchType.Br bbname)
+  | Op.mk "cf.condbr" [vcond] [bbtrue, bbfalse] _ _ _ => do
+        let condval <- Fitree.trigger $ SSAEnvE.Get (MLIRTy.int 32) vcond
+        match condval.down with
+        | 1 => return (BranchType.Br bbtrue)
+        | _ => return (BranchType.Br bbfalse)
+  | _ => do
+      -- TODO: add error messages.
+      Fitree.trigger InvalidOpE.InvalidOp
+      return Option.none
+
+
+
+-- | TODO: generalize so that each dialect can have its effects.
+def cf_semantics_bbstmt {E: Type -> Type}:
+      BasicBlockStmt → Fitree (InvalidOpE +' SSAEnvE +' E) (Option BranchType)
+  | BasicBlockStmt.StmtAssign val _ op => cf_semantics_op op
+  | BasicBlockStmt.StmtOp op => cf_semantics_op op
+
+
+-- | dummy language to check that control flow works correctly.
+def dummy_semantics_op {E: Type -> Type} (ret_name: Option SSAVal): Op → Fitree (InvalidOpE +' SSAEnvE +' E) Unit
+  | Op.mk "dummy.dummy" _ _ _ _ _ => do
+        SSAEnv.set? (MLIRTy.int 32) ret_name 42
+        return ()
+  | Op.mk "dummy.true" _ _ _ _ _ => do
+        SSAEnv.set? (MLIRTy.int 32) ret_name 1
+        return ()
+  | Op.mk "dummy.false" _ _ _ _ _ => do
+        SSAEnv.set? (MLIRTy.int 32) ret_name 0
+        return ()
+  | _ => do
+      -- TODO: add error messages.
+      Fitree.trigger InvalidOpE.InvalidOp
+      return ()
+
+
+def dummy_semantics_bbstmt: BasicBlockStmt ->  Fitree (InvalidOpE +' SSAEnvE +' E) Unit
+| BasicBlockStmt.StmtAssign val _ op => dummy_semantics_op (some val) op
+| BasicBlockStmt.StmtOp op => dummy_semantics_op none op
+
+
+-- | TODO: generalize so that each dialect can have its effects.
+@[simp]
+def cf_semantics_bb {E: Type -> Type} (bb: BasicBlock): Fitree (InvalidOpE +' SSAEnvE +' E) (Option BranchType) := do
+  for stmt in bb.stmts.init do
+     dummy_semantics_bbstmt stmt
+  match bb.stmts.getLast? with
+  | Option.some stmt => cf_semantics_op (stmt.op)
+  | Option.none => return Option.none
+
+-- | The semantics of a region are to use up fuel to run the basic block
+-- | as many times as necessary.
+def cf_semantics_region_go {E: Type -> Type} (fuel: Nat) (r: Region) (bb: BasicBlock):
+  Fitree (InvalidOpE +' SSAEnvE +' E) (Option BranchType) :=
+  match fuel with
+  | 0 => return Option.none
+  | Nat.succ fuel' => do
+          -- | TODO: refactor using OptionT transformer
+          match (<- cf_semantics_bb bb) with
+          | Option.none => return Option.none
+          | Option.some (BranchType.Ret) => return (BranchType.Ret)
+          | Option.some (BranchType.Br bbname) =>
+             let bb? := r.getBasicBlock bbname
+             match bb? with
+             | Option.none => return Option.none
+             | Option.some bb' => cf_semantics_region_go fuel' r bb'
+
+-- | TODO: write a procedure to determine the return type of a region!
+-- | TODO: we need to run some static analysis to find the type of the region o_O ?
+@[simp]
+def cf_semantics_region
+  {E: Type -> Type} (fuel: Nat) (r: Region): Fitree (InvalidOpE +' SSAEnvE +' E) Unit := do
+     let _ <- cf_semantics_region_go fuel r (r.bbs.get! 0)
+
+@[simp]
+def run_cf (t: Fitree (InvalidOpE +' SSAEnvE +' PVoid) Unit) (env: SSAEnv):
+    Fitree PVoid ((Unit × String) × SSAEnv) :=
+  let x := interp_ssa_logged (interp_invalid t sorry)
+  let y := x.run
+  let z := y env
+  z
+
+#check ControlFlowOp
+
+/-
+### Examples and testing
+-/
+
+-- The following extends #reduce with a (skipProofs := true/false) parameter
+-- to not reduce proofs in the kernel. Reducing proofs would cause constant
+-- timeouts, and proofs are used implicitly through well-founded induction for
+-- mutual definitions.
+-- See: https://leanprover.zulipchat.com/#narrow/stream/270676-lean4/topic/Repr.20instance.20for.20functions/near/276504682
+
+open Lean
+open Lean.Parser.Term
+open Lean.Elab.Command
+open Lean.Elab
+open Lean.Meta
+
+elab "#reduce " skipProofs:group(atomic("(" &"skipProofs") " := " (trueVal <|> falseVal) ")") term:term : command =>
+  let skipProofs := skipProofs[3].isOfKind ``trueVal
+  withoutModifyingEnv <| runTermElabM (some `_check) fun _ => do
+    -- dbg_trace term
+    let e ← Term.elabTerm term none
+    Term.synthesizeSyntheticMVarsNoPostponing
+    let (e, _) ← Term.levelMVarToParam (← instantiateMVars e)
+    withTheReader Core.Context (fun ctx => { ctx with options := ctx.options.setBool `smartUnfolding false }) do
+      let e ← withTransparency (mode := TransparencyMode.all) <| reduce e (skipProofs := skipProofs) (skipTypes := false)
+      logInfo e
+
+---
+
+def dummy_stmt := [mlir_bb_stmt|
+  %dummy = "dummy.dummy"() : ()
+]
+
+#reduce (skipProofs := true)
+  dummy_semantics_bbstmt dummy_stmt
+
+
+def true_stmt := [mlir_bb_stmt|
+  %true = "dummy.true"() : ()
+]
+
+#reduce (skipProofs := true)
+  dummy_semantics_bbstmt true_stmt
+
+
+def false_stmt := [mlir_bb_stmt|
+  %false = "dummy.false"() : ()
+]
+#reduce (skipProofs := true)
+  dummy_semantics_bbstmt false_stmt
+
+
+def branch_to_true_region := [mlir_region| {
+  ^entry:
+    %x = "dummy.true"() : ()
+    "cf.condbr"(%x) [^bbtrue, ^bbfalse] : ()
+
+  ^bbtrue:
+    %y = "dummy.dummy" () : ()
+    "ret" () : ()
+
+  ^bbfalse:
+    %z = "dummy.dummy" () : ()
+    "ret" () : ()
+
+}]
+
+
+def run_branch_true : String :=
+  let x := run_cf (cf_semantics_region 5 branch_to_true_region) SSAEnv.empty
+  let y := Fitree.run x
+  y.fst.snd
+
+set_option maxRecDepth 1000
+#eval run_branch_true
+
+
+def branch_to_false_region := [mlir_region| {
+  ^entry:
+    %x = "dummy.false"() : ()
+    "cf.condbr"(%x) [^bbtrue, ^bbfalse] : ()
+    -- "cf.br" () [^bbtrue] : ()
+
+  ^bbtrue:
+    %y = "dummy.dummy" () : ()
+    "ret" () : ()
+
+  ^bbfalse:
+    %z = "dummy.dummy" () : ()
+    "ret" () : ()
+
+}]
+
+#eval branch_to_false_region
+
+def run_branch_false : String :=
+  let x := run_cf (cf_semantics_region 100 branch_to_false_region) SSAEnv.empty
+  let y := Fitree.run x
+  y.fst.snd
+
+set_option maxRecDepth 1000
+#eval run_branch_false
