git/ramonfmir/junglean/JungLean/Impurity.lean
@@ -1,0 +1,40 @@
+import Std.Data.HashMap
+import JungLean.Utils
+
+open Std
+
+variable {α} [BEq α] [Hashable α]
+
+def gini_impur (l : List α) : Float :=
+    let len := l.length
+    let update (tbl : HashMap α Int) i :=
+      if tbl.contains i then tbl.insert i (tbl.find! i + 1)
+      else tbl.insert i 1
+    let tbl := List.foldl (fun tbl i => update tbl i) HashMap.empty l
+    let update :=
+      fun s _ x => s + Float.pow ((Float.ofInt x) / (Float.ofNat len)) 2
+    1 - HashMap.fold update 0 tbl
+
+def split_impur (impur : List α -> Float) (x_labels : List (Float × α)) (thr : Float) : Float :=
+  let append left_right x_l :=
+      let (left, right) := left_right
+      let (x, l) := x_l
+      if x < thr then (l :: left, right) else (left, l :: right)
+  let (left, right) := List.foldl append ([], []) x_labels
+  ((impur left) + (impur right)) / 2.0
+
+def best_split (impur : List α -> Float) (x : List Float) (labels : List α) : Float × Float :=
+    let x_l := List.zip x labels
+    let x_l := sort (fun (a, _) (b, _) => a ≤ b) x_l
+    let rec loop remaining_x_l best_thr best_impur :=
+        match remaining_x_l with
+        | [] => (best_thr, best_impur)
+        | [_] => (best_thr, best_impur)
+        | (x1, l1) :: (x2, l2) :: t =>
+            let new_thr := (x1 + x2) / 2
+            let new_impur := split_impur impur x_l new_thr
+            if new_impur < best_impur then
+                loop ((x2, l2) :: t) new_thr new_impur
+            else
+                loop ((x2, l2) :: t) best_thr best_impur
+    loop x_l 0 1
