git/ramonfmir/junglean/JungLean/Utils.lean
@@ -1,10 +1,10 @@
-/- Ported from: 
+/- Ported from:
 https://github.com/BartoszPiotrowski/random-forest/blob/main/src/utils.ml
 -/
 
 import Init.Data.Random
 
-section List 
+section List
 
 variable {α} [Inhabited α]
 
@@ -16,42 +16,54 @@ def maxList [LT α] [DecidableRel (@LT.lt α _)] : List α → α
   | []         => panic! "Empty list"
   | l@(h :: _) => l.foldl max h
 
-def accuracy [DecidableEq α] (l₁ l₂ : List α) : Float := 
-  assert! l₁.length = l₂.length 
-  let pairs := List.zip l₁ l₂ 
+def accuracy [DecidableEq α] (l₁ l₂ : List α) : Float :=
+  assert! l₁.length = l₂.length
+  let pairs := List.zip l₁ l₂
   let correct := pairs.filter (fun (x, y) => x = y)
   (Float.ofNat correct.length) / (Float.ofNat pairs.length)
 
-def arraySubset (x : List α) (inds : List Nat) : Array α := 
+def arraySubset (x : List α) (inds : List Nat) : Array α :=
   Array.mk $ inds.map (fun i => x.get! i)
 
-def sampleWithReplace (l : List α) (n : Nat) : IO (List α) := 
+def sampleWithReplace (l : List α) (n : Nat) : IO (List α) :=
   let a := Array.mk l
-  let rec loop i r := 
-    match i with 
+  let rec loop i r :=
+    match i with
     | 0 => return r
     | k + 1 => do loop k $ a.get! (← IO.rand 0 (a.size - 1)) :: r
   loop n []
 
 def sample (l : List α) (n : Nat) : IO (List α) :=
   if l.length < n then panic! "List shorter than n" else do
-    let mut a := Array.mk l 
-    for i in List.range n do 
+    let mut a := Array.mk l
+    for i in List.range n do
       let j ← IO.rand 0 (a.size - i - 1)
       let e := a.get! (i + j)
       a := a.set! (i + j) (a.get! i)
-      a := a.set! i e 
+      a := a.set! i e
     return (a.extract 0 n).data
 
-def chooseRandom (l : List α) : IO α := do 
+def chooseRandom (l : List α) : IO α := do
   return l.get! (← IO.rand 0 (l.length - 1))
 
-end List 
+def insert (compare : α → α → Bool) (x : α) (l : List α) : (List α) :=
+  match l with
+  | [] => [x]
+  | h :: t => if compare x h then x :: h :: t else h :: insert compare x t
+
+-- TODO better sorting algo
+def sort (compare : α → α → Bool) (l : List α) : (List α) :=
+  let rec loop : List α → List α → List α
+    | acc, [] => acc
+    | acc, h :: t => loop (insert compare h acc) t
+  loop [] l
+
+end List
 
 def readLines (path : String) : IO (List String) := do
   let handle ← IO.FS.Handle.mk path IO.FS.Mode.read
   let content ← handle.readToEnd
   return (content.splitOn "\n")
 
-def time (f : α → β) (x : α) : IO β := do 
+def time (f : α → β) (x : α) : IO β := do
   timeit "Execution time: " (return f x)
