git/siddhartha-gadgil/Polylean/Polylean/TorsionFree.lean
@@ -1,0 +1,71 @@
+import Polylean.GardamGroup
+
+/-
+This file contains a proof that the group `P` defined is in fact torsion-free.
+
+Roughly, the steps are as follows (further details can be found in the corresponding `.md` file):
+1. Define a function `s : Q -> K -> K` taking a group element `(q, k)` to its square `(s q k, 0)`. This element lies in the kernel as the group `ℤ₂ × ℤ₂` is annihilated by `2`.
+2. Show that elements of the form `((a, b, c), (0, 0))` do not have torsion. This argument requires proving (something very close to) the fact that `ℤ` is an integral domain.
+3. Show that no element of `P` has order precisely `2`. This is an argument by cases on the `Q` part of elements of `P`.
+4. Finally, if an element `g : P` is in the kernel of the `n`-th power homomorphism, then so is `g^2`. But from the above statements, we see that `g^2` is of the form `(k, 0)` and hence
+   either `g^2 = e` or `n = 0` (as elements of this form cannot have torsion). If `g^2 = e`, then `g = e` as `P` does not contain any order `2` elements. Otherwise, `n = 0`.
+5. Together, this shows that `P` is torsion-free.
+-/
+
+open P
+
+def s : K → Q → K
+  | (p, q, r), (0, 0) => (p + p, q + q, r + r)
+  | (p, q, r), (0, 1) => (0, q + q + 1, 0)
+  | (p, q, r), (1, 0) => (p + p + 1, 0, 0)
+  | (p, q, r), (1, 1) => (0, 0, r + r + 1)
+
+theorem s_square : ∀ g : P, g ^ 2 = (s g.fst g.snd, 0) := by
+  intro ((p, q, r), x)
+  revert x
+  apply Q.rec <;> simp [s] -- unable to simplify the multiplication
+  · sorry
+  · sorry
+  · sorry
+  · sorry
+
+-- needs slight rewording
+def torsion_free (G : Type _) [Group G] (g : G) := ∀ n : ℕ, g ^ n.succ = 1 → g = 1
+
+-- this is the most difficult part of the argument
+theorem kernel_torsion_free : ∀  k : K, torsion_free P (k, 0) := sorry
+
+theorem square_free : ∀ g : P, g ^ 2 = 1 → g = 1 := by
+  intro ⟨k, q⟩
+  revert q
+  have sq (g : P) : g ^ 2 = g * g :=  by rw [← npow_eq_pow]; simp [Monoid.npow, npow_rec]
+  apply Q.rec (λ q => (k, q) ^ 2 = (0, 0) → (k, q) = (0, 0))
+  <;> intro hyp <;> simp
+  · let g : P := (k, 0)
+    have metabelian_mul : g * g = (k + (0 : Q) • k + cocycle 0 0, 0) := rfl
+    rw [P_cocycle.cocycleId, add_zero, P_action.id_action] at metabelian_mul
+    have : g = (k, (⟨0, by decide⟩, ⟨0, by decide⟩))  := rfl
+    rw [← this, sq] at hyp
+    have sq : g * (g * 1) = g ^ 2 := rfl
+    have : k + k = 0 := congrArg Prod.fst (Eq.trans (Eq.symm metabelian_mul) hyp)
+    sorry -- deducing `k = 0` requires the fact that `K` is torsion-free
+  · sorry
+  · sorry
+  · sorry
+
+theorem torsion_implies_square_torsion : ∀ g : P, ∀ n : ℕ, g ^ n = 1 → (g ^ 2) ^ n = 1 :=
+  λ g n g_tor =>
+    calc (g ^ 2) ^ n = g ^ (2 * n) := by rw [← pow_mul]
+              _      = g ^ (n * 2) := by rw [mul_comm]
+              _      = (g ^ n) ^ 2 := by rw [pow_mul]
+              _      = (1 : P) ^ 2 := by rw [← g_tor]
+              _      = (1 : P)     := rfl
+
+  theorem P_torsion_free : ∀ g : P, torsion_free P g := by
+    intros g n g_tor
+    have square_tor : (g ^ 2) ^ n.succ = 1 := torsion_implies_square_torsion g n.succ g_tor
+    have square_eq : g ^ 2 = (s g.fst g.snd, 0) := s_square g
+    rw [square_eq] at square_tor
+    have square_zero : (s g.fst g.snd, 0) = ((0, 0) : P) := kernel_torsion_free (s g.fst g.snd) n square_tor
+    rw [← s_square] at square_zero
+    exact square_free g square_zero
